<?xml version="1.0"?>
<rdf:RDF xmlns="https://w3id.org/digitalconstruction/0.5/Entities#"
     xml:base="https://w3id.org/digitalconstruction/0.5/Entities"
     xmlns:dc="http://purl.org/dc/elements/1.1/"
     xmlns:owl="http://www.w3.org/2002/07/owl#"
     xmlns:rdf="http://www.w3.org/1999/02/22-rdf-syntax-ns#"
     xmlns:xml="http://www.w3.org/XML/1998/namespace"
     xmlns:xsd="http://www.w3.org/2001/XMLSchema#"
     xmlns:dicc="https://w3id.org/digitalconstruction/0.5/Contexts#"
     xmlns:dicv="https://w3id.org/digitalconstruction/0.5/Variables#"
     xmlns:obda="https://w3id.org/obda/vocabulary#"
     xmlns:rdfs="http://www.w3.org/2000/01/rdf-schema#"
     xmlns:vann="http://purl.org/vocab/vann/"
     xmlns:terms="http://purl.org/dc/terms/">
    <owl:Ontology rdf:about="https://w3id.org/digitalconstruction/0.5/Entities">
        <owl:imports rdf:resource="https://w3id.org/digitalconstruction/0.5/Contexts/contexts.ttl"/>
        <dc:date>2021-03-31</dc:date>
        <dc:title>Digital Construction Entities</dc:title>
        <terms:created>2020-01-12</terms:created>
        <terms:creator>Seppo Törmä</terms:creator>
        <terms:creator>Yuan Zheng</terms:creator>
        <terms:license rdf:resource="https://creativecommons.org/licenses/by/4.0/"/>
        <vann:preferredNamespacePrefix>dice</vann:preferredNamespacePrefix>
        <vann:preferredNamespaceUri>https://w3id.org/digitalconstruction/0.5/Entities</vann:preferredNamespaceUri>
        <rdfs:comment>Digital Construction Entities Ontology defines the basic classes and properties needed for the representation of construction and renovation projects. Examples are building object, location, material batch, equipment, agent, information content entity, activity and related time concepts. The ontology is based on BFO. </rdfs:comment>
        <rdfs:label>Digital Construction Entities</rdfs:label>
        <rdfs:seeAlso rdf:resource="https://w3id.org/digitalconstruction/0.5/"/>
    </owl:Ontology>
    


    <!-- 
    ///////////////////////////////////////////////////////////////////////////////////////
    //
    // Annotation properties
    //
    ///////////////////////////////////////////////////////////////////////////////////////
     -->

    


    <!-- http://purl.org/dc/elements/1.1/creator -->

    <owl:AnnotationProperty rdf:about="http://purl.org/dc/elements/1.1/creator"/>
    


    <!-- http://purl.org/dc/elements/1.1/date -->

    <owl:AnnotationProperty rdf:about="http://purl.org/dc/elements/1.1/date"/>
    


    <!-- http://purl.org/dc/elements/1.1/title -->

    <owl:AnnotationProperty rdf:about="http://purl.org/dc/elements/1.1/title"/>
    


    <!-- http://purl.org/dc/terms/abstract -->

    <owl:AnnotationProperty rdf:about="http://purl.org/dc/terms/abstract"/>
    


    <!-- http://purl.org/dc/terms/created -->

    <owl:AnnotationProperty rdf:about="http://purl.org/dc/terms/created"/>
    


    <!-- http://purl.org/dc/terms/creator -->

    <owl:AnnotationProperty rdf:about="http://purl.org/dc/terms/creator"/>
    


    <!-- http://purl.org/dc/terms/description -->

    <owl:AnnotationProperty rdf:about="http://purl.org/dc/terms/description"/>
    


    <!-- http://purl.org/dc/terms/license -->

    <owl:AnnotationProperty rdf:about="http://purl.org/dc/terms/license"/>
    


    <!-- http://purl.org/vocab/vann/preferredNamespacePrefix -->

    <owl:AnnotationProperty rdf:about="http://purl.org/vocab/vann/preferredNamespacePrefix"/>
    


    <!-- http://purl.org/vocab/vann/preferredNamespaceUri -->

    <owl:AnnotationProperty rdf:about="http://purl.org/vocab/vann/preferredNamespaceUri"/>
    


    <!-- 
    ///////////////////////////////////////////////////////////////////////////////////////
    //
    // Object Properties
    //
    ///////////////////////////////////////////////////////////////////////////////////////
     -->

    


    <!-- https://w3id.org/digitalconstruction/0.5/Entities#assignsInstanceTo -->

    <owl:ObjectProperty rdf:about="https://w3id.org/digitalconstruction/0.5/Entities#assignsInstanceTo">
        <rdfs:subPropertyOf rdf:resource="https://w3id.org/digitalconstruction/0.5/Entities#identifies"/>
        <owl:inverseOf rdf:resource="https://w3id.org/digitalconstruction/0.5/Entities#isAssignedToInstance"/>
        <rdfs:domain rdf:resource="https://w3id.org/digitalconstruction/0.5/Entities#Identifier"/>
        <rdfs:range rdf:resource="https://w3id.org/digitalconstruction/0.5/Entities#MaterialEntity"/>
        <rdfs:label>assignsInstanceTo</rdfs:label>
    </owl:ObjectProperty>
    


    <!-- https://w3id.org/digitalconstruction/0.5/Entities#assignsTypeTo -->

    <owl:ObjectProperty rdf:about="https://w3id.org/digitalconstruction/0.5/Entities#assignsTypeTo">
        <rdfs:subPropertyOf rdf:resource="https://w3id.org/digitalconstruction/0.5/Entities#classifies"/>
        <owl:inverseOf rdf:resource="https://w3id.org/digitalconstruction/0.5/Entities#isAssignedToType"/>
        <rdfs:domain rdf:resource="https://w3id.org/digitalconstruction/0.5/Entities#Category"/>
        <rdfs:range rdf:resource="https://w3id.org/digitalconstruction/0.5/Entities#MaterialEntity"/>
        <rdfs:comment>Assignment of a selected type to an entity. An example is product assignment.</rdfs:comment>
        <rdfs:label>assignsTypeTo</rdfs:label>
    </owl:ObjectProperty>
    


    <!-- https://w3id.org/digitalconstruction/0.5/Entities#bearerOf -->

    <owl:ObjectProperty rdf:about="https://w3id.org/digitalconstruction/0.5/Entities#bearerOf">
        <rdfs:subPropertyOf rdf:resource="https://w3id.org/digitalconstruction/0.5/Entities#specificallyDependedOnBy"/>
        <rdfs:domain>
            <owl:Class>
                <owl:intersectionOf rdf:parseType="Collection">
                    <rdf:Description rdf:about="https://w3id.org/digitalconstruction/0.5/Entities#IndependentContinuant"/>
                    <owl:Class>
                        <owl:complementOf rdf:resource="https://w3id.org/digitalconstruction/0.5/Entities#SpatialRegion"/>
                    </owl:Class>
                </owl:intersectionOf>
            </owl:Class>
        </rdfs:domain>
        <rdfs:range rdf:resource="https://w3id.org/digitalconstruction/0.5/Entities#SpecificallyDependentContinuant"/>
        <rdfs:comment>bearerOf is equivalent to the BFO property &apos;bearer of&apos; (http://purl.obolibrary.org/obo/BFO_0000196)</rdfs:comment>
        <rdfs:label>bearerOf</rdfs:label>
    </owl:ObjectProperty>
    


    <!-- https://w3id.org/digitalconstruction/0.5/Entities#belongsTo -->

    <owl:ObjectProperty rdf:about="https://w3id.org/digitalconstruction/0.5/Entities#belongsTo">
        <rdfs:subPropertyOf rdf:resource="https://w3id.org/digitalconstruction/0.5/Entities#labeledBy"/>
        <owl:inverseOf rdf:resource="https://w3id.org/digitalconstruction/0.5/Entities#categorises"/>
        <rdfs:label>belongsTo</rdfs:label>
    </owl:ObjectProperty>
    


    <!-- https://w3id.org/digitalconstruction/0.5/Entities#categorises -->

    <owl:ObjectProperty rdf:about="https://w3id.org/digitalconstruction/0.5/Entities#categorises">
        <owl:equivalentProperty rdf:resource="https://w3id.org/digitalconstruction/0.5/Entities#classifies"/>
        <rdfs:subPropertyOf rdf:resource="https://w3id.org/digitalconstruction/0.5/Entities#labels"/>
    </owl:ObjectProperty>
    


    <!-- https://w3id.org/digitalconstruction/0.5/Entities#classifies -->

    <owl:ObjectProperty rdf:about="https://w3id.org/digitalconstruction/0.5/Entities#classifies">
        <rdfs:subPropertyOf rdf:resource="https://w3id.org/digitalconstruction/0.5/Entities#labels"/>
        <owl:inverseOf rdf:resource="https://w3id.org/digitalconstruction/0.5/Entities#isClassifiedBy"/>
        <rdfs:domain rdf:resource="https://w3id.org/digitalconstruction/0.5/Entities#Category"/>
        <rdfs:range rdf:resource="https://w3id.org/digitalconstruction/0.5/Entities#Entity"/>
        <rdfs:label>classifies</rdfs:label>
    </owl:ObjectProperty>
    


    <!-- https://w3id.org/digitalconstruction/0.5/Entities#concretizes -->

    <owl:ObjectProperty rdf:about="https://w3id.org/digitalconstruction/0.5/Entities#concretizes">
        <rdfs:domain>
            <owl:Class>
                <owl:unionOf rdf:parseType="Collection">
                    <rdf:Description rdf:about="https://w3id.org/digitalconstruction/0.5/Entities#Process"/>
                    <rdf:Description rdf:about="https://w3id.org/digitalconstruction/0.5/Entities#SpecificallyDependentContinuant"/>
                </owl:unionOf>
            </owl:Class>
        </rdfs:domain>
        <rdfs:range rdf:resource="https://w3id.org/digitalconstruction/0.5/Entities#GenericallyDependentContinuant"/>
        <rdfs:comment>concretizes is equivalent to the BFO property &apos;concretizes at some time&apos; (http://purl.obolibrary.org/obo/BFO_0000059)</rdfs:comment>
        <rdfs:label>concretizes</rdfs:label>
    </owl:ObjectProperty>
    


    <!-- https://w3id.org/digitalconstruction/0.5/Entities#concretizesAtAllTimes -->

    <owl:ObjectProperty rdf:about="https://w3id.org/digitalconstruction/0.5/Entities#concretizesAtAllTimes">
        <rdfs:subPropertyOf rdf:resource="https://w3id.org/digitalconstruction/0.5/Entities#concretizes"/>
        <rdfs:domain>
            <owl:Class>
                <owl:unionOf rdf:parseType="Collection">
                    <rdf:Description rdf:about="https://w3id.org/digitalconstruction/0.5/Entities#Process"/>
                    <rdf:Description rdf:about="https://w3id.org/digitalconstruction/0.5/Entities#SpecificallyDependentContinuant"/>
                </owl:unionOf>
            </owl:Class>
        </rdfs:domain>
        <rdfs:range rdf:resource="https://w3id.org/digitalconstruction/0.5/Entities#GenericallyDependentContinuant"/>
        <rdfs:comment>concretizesAtAllTimes is equivalent to the BFO property &apos;concretizes at all times&apos; (http://purl.obolibrary.org/obo/BFO_0000164)</rdfs:comment>
        <rdfs:label>concretizesAtAllTimes</rdfs:label>
    </owl:ObjectProperty>
    


    <!-- https://w3id.org/digitalconstruction/0.5/Entities#containsIdentifiedEntities -->

    <owl:ObjectProperty rdf:about="https://w3id.org/digitalconstruction/0.5/Entities#containsIdentifiedEntities">
        <owl:inverseOf rdf:resource="https://w3id.org/digitalconstruction/0.5/Entities#hasEntitiesFrom"/>
        <rdfs:domain rdf:resource="https://w3id.org/digitalconstruction/0.5/Entities#Entity"/>
        <rdfs:range rdf:resource="https://w3id.org/digitalconstruction/0.5/Entities#EntityScope"/>
        <rdfs:label>containsIdentifiedEntities</rdfs:label>
    </owl:ObjectProperty>
    


    <!-- https://w3id.org/digitalconstruction/0.5/Entities#continuantPartOf -->

    <owl:ObjectProperty rdf:about="https://w3id.org/digitalconstruction/0.5/Entities#continuantPartOf">
        <rdfs:subPropertyOf rdf:resource="https://w3id.org/digitalconstruction/0.5/Entities#isPartOf"/>
        <rdfs:domain rdf:resource="https://w3id.org/digitalconstruction/0.5/Entities#Continuant"/>
        <rdfs:range rdf:resource="https://w3id.org/digitalconstruction/0.5/Entities#Continuant"/>
        <rdfs:comment>continuantPartOf is equivalent to the BFO property &apos;continuant part of at some time&apos; (http://purl.obolibrary.org/obo/BFO_0000176)</rdfs:comment>
        <rdfs:label>continuantPartOf</rdfs:label>
    </owl:ObjectProperty>
    


    <!-- https://w3id.org/digitalconstruction/0.5/Entities#continuantPartOfAtAllTimes -->

    <owl:ObjectProperty rdf:about="https://w3id.org/digitalconstruction/0.5/Entities#continuantPartOfAtAllTimes">
        <rdfs:subPropertyOf rdf:resource="https://w3id.org/digitalconstruction/0.5/Entities#continuantPartOf"/>
        <rdf:type rdf:resource="http://www.w3.org/2002/07/owl#TransitiveProperty"/>
        <rdfs:domain rdf:resource="https://w3id.org/digitalconstruction/0.5/Entities#Continuant"/>
        <rdfs:range rdf:resource="https://w3id.org/digitalconstruction/0.5/Entities#Continuant"/>
        <rdfs:comment>continuantPartOfAtAllTimes is equivalent to the BFO property &apos;continuant part of at all times&apos; (http://purl.obolibrary.org/obo/BFO_0000177)</rdfs:comment>
        <rdfs:label>continuantPartOfAtAllTimes</rdfs:label>
    </owl:ObjectProperty>
    


    <!-- https://w3id.org/digitalconstruction/0.5/Entities#environs -->

    <owl:ObjectProperty rdf:about="https://w3id.org/digitalconstruction/0.5/Entities#environs">
        <rdfs:domain>
            <owl:Class>
                <owl:unionOf rdf:parseType="Collection">
                    <rdf:Description rdf:about="https://w3id.org/digitalconstruction/0.5/Entities#MaterialEntity"/>
                    <rdf:Description rdf:about="https://w3id.org/digitalconstruction/0.5/Entities#Site"/>
                </owl:unionOf>
            </owl:Class>
        </rdfs:domain>
        <rdfs:range>
            <owl:Class>
                <owl:unionOf rdf:parseType="Collection">
                    <rdf:Description rdf:about="https://w3id.org/digitalconstruction/0.5/Entities#Process"/>
                    <rdf:Description rdf:about="https://w3id.org/digitalconstruction/0.5/Entities#ProcessBoundary"/>
                </owl:unionOf>
            </owl:Class>
        </rdfs:range>
        <rdfs:comment>environs is equivalent to the BFO property &apos;environs&apos; (http://purl.obolibrary.org/obo/BFO_0000183)</rdfs:comment>
        <rdfs:label>environs</rdfs:label>
    </owl:ObjectProperty>
    


    <!-- https://w3id.org/digitalconstruction/0.5/Entities#existsAt -->

    <owl:ObjectProperty rdf:about="https://w3id.org/digitalconstruction/0.5/Entities#existsAt">
        <rdfs:comment>existsAt is equivalent to the BFO property &apos;exists at&apos; (http://purl.obolibrary.org/obo/BFO_0000108)</rdfs:comment>
        <rdfs:label>existsAt</rdfs:label>
    </owl:ObjectProperty>
    


    <!-- https://w3id.org/digitalconstruction/0.5/Entities#firstInstantOf -->

    <owl:ObjectProperty rdf:about="https://w3id.org/digitalconstruction/0.5/Entities#firstInstantOf">
        <rdfs:domain rdf:resource="https://w3id.org/digitalconstruction/0.5/Entities#TimeInstant"/>
        <rdfs:range rdf:resource="https://w3id.org/digitalconstruction/0.5/Entities#TemporalRegion"/>
        <rdfs:comment>firstInstantOf is equivalent to the BFO property &apos;first instant of&apos; (http://purl.obolibrary.org/obo/BFO_0000221)</rdfs:comment>
        <rdfs:label>firstInstantOf</rdfs:label>
    </owl:ObjectProperty>
    


    <!-- https://w3id.org/digitalconstruction/0.5/Entities#genericallyDependsOn -->

    <owl:ObjectProperty rdf:about="https://w3id.org/digitalconstruction/0.5/Entities#genericallyDependsOn">
        <rdfs:domain rdf:resource="https://w3id.org/digitalconstruction/0.5/Entities#GenericallyDependentContinuant"/>
        <rdfs:range>
            <owl:Class>
                <owl:intersectionOf rdf:parseType="Collection">
                    <rdf:Description rdf:about="https://w3id.org/digitalconstruction/0.5/Entities#IndependentContinuant"/>
                    <owl:Class>
                        <owl:complementOf rdf:resource="https://w3id.org/digitalconstruction/0.5/Entities#SpatialRegion"/>
                    </owl:Class>
                </owl:intersectionOf>
            </owl:Class>
        </rdfs:range>
        <rdfs:comment>genericallyDependsOn is equivalent to the BFO property &apos;generically depends on at some time&apos; (http://purl.obolibrary.org/obo/BFO_0000084)</rdfs:comment>
        <rdfs:label>genericallyDependsOn</rdfs:label>
    </owl:ObjectProperty>
    


    <!-- https://w3id.org/digitalconstruction/0.5/Entities#genericallyDependsOnAtAllTimes -->

    <owl:ObjectProperty rdf:about="https://w3id.org/digitalconstruction/0.5/Entities#genericallyDependsOnAtAllTimes">
        <rdfs:subPropertyOf rdf:resource="https://w3id.org/digitalconstruction/0.5/Entities#genericallyDependsOn"/>
        <rdfs:domain rdf:resource="https://w3id.org/digitalconstruction/0.5/Entities#GenericallyDependentContinuant"/>
        <rdfs:range>
            <owl:Class>
                <owl:intersectionOf rdf:parseType="Collection">
                    <rdf:Description rdf:about="https://w3id.org/digitalconstruction/0.5/Entities#IndependentContinuant"/>
                    <owl:Class>
                        <owl:complementOf rdf:resource="https://w3id.org/digitalconstruction/0.5/Entities#SpatialRegion"/>
                    </owl:Class>
                </owl:intersectionOf>
            </owl:Class>
        </rdfs:range>
        <rdfs:comment>genericallyDependsOnAtAllTimes is equivalent to the BFO property &apos;generically depends on at all times&apos; (http://purl.obolibrary.org/obo/BFO_0000219)</rdfs:comment>
        <rdfs:label>genericallyDependsOnAtAllTimes</rdfs:label>
    </owl:ObjectProperty>
    


    <!-- https://w3id.org/digitalconstruction/0.5/Entities#hasAdjacentElement -->

    <owl:ObjectProperty rdf:about="https://w3id.org/digitalconstruction/0.5/Entities#hasAdjacentElement">
        <rdf:type rdf:resource="http://www.w3.org/2002/07/owl#SymmetricProperty"/>
        <rdfs:domain rdf:resource="https://w3id.org/digitalconstruction/0.5/Entities#IndependentContinuant"/>
        <rdfs:range rdf:resource="https://w3id.org/digitalconstruction/0.5/Entities#IndependentContinuant"/>
        <rdfs:label>hasAdjacentElement</rdfs:label>
    </owl:ObjectProperty>
    


    <!-- https://w3id.org/digitalconstruction/0.5/Entities#hasBuilding -->

    <owl:ObjectProperty rdf:about="https://w3id.org/digitalconstruction/0.5/Entities#hasBuilding">
        <owl:inverseOf rdf:resource="https://w3id.org/digitalconstruction/0.5/Entities#isBuildingOf"/>
        <rdfs:domain rdf:resource="https://w3id.org/digitalconstruction/0.5/Entities#RealEstate"/>
        <rdfs:range rdf:resource="https://w3id.org/digitalconstruction/0.5/Entities#Building"/>
        <rdfs:label>hasBuilding</rdfs:label>
    </owl:ObjectProperty>
    


    <!-- https://w3id.org/digitalconstruction/0.5/Entities#hasBuildingUnit -->

    <owl:ObjectProperty rdf:about="https://w3id.org/digitalconstruction/0.5/Entities#hasBuildingUnit">
        <owl:inverseOf rdf:resource="https://w3id.org/digitalconstruction/0.5/Entities#isBuildingUnitOf"/>
        <rdfs:domain rdf:resource="https://w3id.org/digitalconstruction/0.5/Entities#Building"/>
        <rdfs:range rdf:resource="https://w3id.org/digitalconstruction/0.5/Entities#BuildingUnit"/>
        <rdfs:label>hasBuildingUnit</rdfs:label>
    </owl:ObjectProperty>
    


    <!-- https://w3id.org/digitalconstruction/0.5/Entities#hasCapability -->

    <owl:ObjectProperty rdf:about="https://w3id.org/digitalconstruction/0.5/Entities#hasCapability">
        <rdfs:subPropertyOf rdf:resource="https://w3id.org/digitalconstruction/0.5/Entities#bearerOf"/>
        <owl:inverseOf rdf:resource="https://w3id.org/digitalconstruction/0.5/Entities#isCapabilityOf"/>
        <rdfs:domain rdf:resource="https://w3id.org/digitalconstruction/0.5/Entities#MaterialEntity"/>
        <rdfs:range rdf:resource="https://w3id.org/digitalconstruction/0.5/Entities#Capability"/>
        <rdfs:label>hasCapability</rdfs:label>
    </owl:ObjectProperty>
    


    <!-- https://w3id.org/digitalconstruction/0.5/Entities#hasContinuantPart -->

    <owl:ObjectProperty rdf:about="https://w3id.org/digitalconstruction/0.5/Entities#hasContinuantPart">
        <rdfs:subPropertyOf rdf:resource="https://w3id.org/digitalconstruction/0.5/Entities#hasPart"/>
        <rdfs:domain rdf:resource="https://w3id.org/digitalconstruction/0.5/Entities#Continuant"/>
        <rdfs:range rdf:resource="https://w3id.org/digitalconstruction/0.5/Entities#Continuant"/>
        <rdfs:comment>hasContinuantPart is equivalent to the BFO property &apos;has continuant part at some time&apos; (http://purl.obolibrary.org/obo/BFO_0000178)</rdfs:comment>
        <rdfs:label>hasContinuantPart</rdfs:label>
    </owl:ObjectProperty>
    


    <!-- https://w3id.org/digitalconstruction/0.5/Entities#hasContinuantPartAtAllTimes -->

    <owl:ObjectProperty rdf:about="https://w3id.org/digitalconstruction/0.5/Entities#hasContinuantPartAtAllTimes">
        <rdfs:subPropertyOf rdf:resource="https://w3id.org/digitalconstruction/0.5/Entities#hasContinuantPart"/>
        <rdf:type rdf:resource="http://www.w3.org/2002/07/owl#TransitiveProperty"/>
        <rdfs:domain rdf:resource="https://w3id.org/digitalconstruction/0.5/Entities#Continuant"/>
        <rdfs:range rdf:resource="https://w3id.org/digitalconstruction/0.5/Entities#Continuant"/>
        <rdfs:comment>hasContinuantPartAtAllTimes is equivalent to the BFO property &apos;has continuant part at all times&apos; (http://purl.obolibrary.org/obo/BFO_0000110)</rdfs:comment>
        <rdfs:label>hasContinuantPartAtAllTimes</rdfs:label>
    </owl:ObjectProperty>
    


    <!-- https://w3id.org/digitalconstruction/0.5/Entities#hasDetermined -->

    <owl:ObjectProperty rdf:about="https://w3id.org/digitalconstruction/0.5/Entities#hasDetermined">
        <owl:inverseOf rdf:resource="https://w3id.org/digitalconstruction/0.5/Entities#isDeterminedBy"/>
        <rdfs:domain rdf:resource="https://w3id.org/digitalconstruction/0.5/Entities#MaterialEntity"/>
        <rdfs:range rdf:resource="https://w3id.org/digitalconstruction/0.5/Variables#PropertyState"/>
        <rdfs:comment>The property state(s) that have been determined by a material entity (an agent or a sensor).</rdfs:comment>
        <rdfs:label>hasDetermined</rdfs:label>
    </owl:ObjectProperty>
    


    <!-- https://w3id.org/digitalconstruction/0.5/Entities#hasDuration -->

    <owl:ObjectProperty rdf:about="https://w3id.org/digitalconstruction/0.5/Entities#hasDuration">
        <rdfs:domain rdf:resource="https://w3id.org/digitalconstruction/0.5/Entities#TimeInterval"/>
        <rdfs:range rdf:resource="https://w3id.org/digitalconstruction/0.5/Entities#TimeDuration"/>
        <rdfs:label>hasDuration</rdfs:label>
    </owl:ObjectProperty>
    


    <!-- https://w3id.org/digitalconstruction/0.5/Entities#hasEnd -->

    <owl:ObjectProperty rdf:about="https://w3id.org/digitalconstruction/0.5/Entities#hasEnd">
        <rdfs:subPropertyOf rdf:resource="https://w3id.org/digitalconstruction/0.5/Entities#hasLastInstant"/>
        <owl:inverseOf rdf:resource="https://w3id.org/digitalconstruction/0.5/Entities#isEndOf"/>
        <rdfs:domain rdf:resource="https://w3id.org/digitalconstruction/0.5/Entities#TimeInterval"/>
        <rdfs:range rdf:resource="https://w3id.org/digitalconstruction/0.5/Entities#TimeInstant"/>
        <rdfs:label>hasEnd</rdfs:label>
    </owl:ObjectProperty>
    


    <!-- https://w3id.org/digitalconstruction/0.5/Entities#hasEntitiesFrom -->

    <owl:ObjectProperty rdf:about="https://w3id.org/digitalconstruction/0.5/Entities#hasEntitiesFrom">
        <rdfs:domain rdf:resource="https://w3id.org/digitalconstruction/0.5/Entities#EntityScope"/>
        <rdfs:range rdf:resource="https://w3id.org/digitalconstruction/0.5/Entities#Entity"/>
        <rdfs:label>hasEntitiesFrom</rdfs:label>
    </owl:ObjectProperty>
    


    <!-- https://w3id.org/digitalconstruction/0.5/Entities#hasEntityState -->

    <owl:ObjectProperty rdf:about="https://w3id.org/digitalconstruction/0.5/Entities#hasEntityState">
        <owl:inverseOf rdf:resource="https://w3id.org/digitalconstruction/0.5/Entities#isEntityStateOf"/>
        <rdfs:domain rdf:resource="https://w3id.org/digitalconstruction/0.5/Entities#Entity"/>
        <rdfs:range rdf:resource="https://w3id.org/digitalconstruction/0.5/Entities#EntityState"/>
        <rdfs:comment>State of an entity</rdfs:comment>
        <rdfs:label>hasEntityState</rdfs:label>
    </owl:ObjectProperty>
    


    <!-- https://w3id.org/digitalconstruction/0.5/Entities#hasEquipment -->

    <owl:ObjectProperty rdf:about="https://w3id.org/digitalconstruction/0.5/Entities#hasEquipment">
        <rdfs:subPropertyOf rdf:resource="https://w3id.org/digitalconstruction/0.5/Entities#hasParticipant"/>
        <owl:inverseOf rdf:resource="https://w3id.org/digitalconstruction/0.5/Entities#isEquipmentIn"/>
        <rdfs:domain rdf:resource="https://w3id.org/digitalconstruction/0.5/Entities#Process"/>
        <rdfs:range rdf:resource="https://w3id.org/digitalconstruction/0.5/Entities#Equipment"/>
        <rdfs:label>hasEquipment</rdfs:label>
    </owl:ObjectProperty>
    


    <!-- https://w3id.org/digitalconstruction/0.5/Entities#hasFirstInstant -->

    <owl:ObjectProperty rdf:about="https://w3id.org/digitalconstruction/0.5/Entities#hasFirstInstant">
        <rdf:type rdf:resource="http://www.w3.org/2002/07/owl#FunctionalProperty"/>
        <rdfs:domain rdf:resource="https://w3id.org/digitalconstruction/0.5/Entities#TemporalRegion"/>
        <rdfs:range rdf:resource="https://w3id.org/digitalconstruction/0.5/Entities#TimeInstant"/>
        <rdfs:comment>hasFirstInstant is equivalent to the BFO property &apos;has first instant&apos; (http://purl.obolibrary.org/obo/BFO_0000222)</rdfs:comment>
        <rdfs:label>hasFirstInstant</rdfs:label>
    </owl:ObjectProperty>
    


    <!-- https://w3id.org/digitalconstruction/0.5/Entities#hasHistory -->

    <owl:ObjectProperty rdf:about="https://w3id.org/digitalconstruction/0.5/Entities#hasHistory">
        <rdfs:domain rdf:resource="https://w3id.org/digitalconstruction/0.5/Entities#MaterialEntity"/>
        <rdfs:range rdf:resource="https://w3id.org/digitalconstruction/0.5/Entities#History"/>
        <rdfs:comment>hasHistory is equivalent to the BFO property &apos;has history&apos; (http://purl.obolibrary.org/obo/BFO_0000185)</rdfs:comment>
        <rdfs:label>hasHistory</rdfs:label>
    </owl:ObjectProperty>
    


    <!-- https://w3id.org/digitalconstruction/0.5/Entities#hasLastInstant -->

    <owl:ObjectProperty rdf:about="https://w3id.org/digitalconstruction/0.5/Entities#hasLastInstant">
        <rdf:type rdf:resource="http://www.w3.org/2002/07/owl#FunctionalProperty"/>
        <rdfs:domain rdf:resource="https://w3id.org/digitalconstruction/0.5/Entities#TemporalRegion"/>
        <rdfs:range rdf:resource="https://w3id.org/digitalconstruction/0.5/Entities#TimeInstant"/>
        <rdfs:comment>hasLastInstant is equivalent to the BFO property &apos;has last instant&apos; (http://purl.obolibrary.org/obo/BFO_0000224)</rdfs:comment>
        <rdfs:label>hasLastInstant</rdfs:label>
    </owl:ObjectProperty>
    


    <!-- https://w3id.org/digitalconstruction/0.5/Entities#hasLocationAtAllTimes -->

    <owl:ObjectProperty rdf:about="https://w3id.org/digitalconstruction/0.5/Entities#hasLocationAtAllTimes"/>
    


    <!-- https://w3id.org/digitalconstruction/0.5/Entities#hasMaterialBasis -->

    <owl:ObjectProperty rdf:about="https://w3id.org/digitalconstruction/0.5/Entities#hasMaterialBasis">
        <rdfs:domain rdf:resource="https://w3id.org/digitalconstruction/0.5/Entities#Disposition"/>
        <rdfs:range rdf:resource="https://w3id.org/digitalconstruction/0.5/Entities#MaterialEntity"/>
        <rdfs:comment>hasMaterialBasis is equivalent to the BFO property &apos;has material basis at some time&apos; (http://purl.obolibrary.org/obo/BFO_0000218)</rdfs:comment>
        <rdfs:label>hasMaterialBasis</rdfs:label>
    </owl:ObjectProperty>
    


    <!-- https://w3id.org/digitalconstruction/0.5/Entities#hasMaterialBasisAtAllTimes -->

    <owl:ObjectProperty rdf:about="https://w3id.org/digitalconstruction/0.5/Entities#hasMaterialBasisAtAllTimes">
        <rdfs:subPropertyOf rdf:resource="https://w3id.org/digitalconstruction/0.5/Entities#hasMaterialBasis"/>
        <rdfs:domain rdf:resource="https://w3id.org/digitalconstruction/0.5/Entities#Disposition"/>
        <rdfs:range rdf:resource="https://w3id.org/digitalconstruction/0.5/Entities#MaterialEntity"/>
        <rdfs:comment>hasMaterialBasisAtAllTimes is equivalent to the BFO property &apos;has material basis at all times&apos; (http://purl.obolibrary.org/obo/BFO_0000113)</rdfs:comment>
        <rdfs:label>hasMaterialBasisAtAllTimes</rdfs:label>
    </owl:ObjectProperty>
    


    <!-- https://w3id.org/digitalconstruction/0.5/Entities#hasMaximumCartesianPosition -->

    <owl:ObjectProperty rdf:about="https://w3id.org/digitalconstruction/0.5/Entities#hasMaximumCartesianPosition">
        <rdfs:domain rdf:resource="https://w3id.org/digitalconstruction/0.5/Entities#CartesianBoundingBox"/>
        <rdfs:range rdf:resource="https://w3id.org/digitalconstruction/0.5/Entities#CartesianPosition"/>
        <rdfs:label>hasMaximumCartesianPosition</rdfs:label>
    </owl:ObjectProperty>
    


    <!-- https://w3id.org/digitalconstruction/0.5/Entities#hasMaximumGeodeticPosition -->

    <owl:ObjectProperty rdf:about="https://w3id.org/digitalconstruction/0.5/Entities#hasMaximumGeodeticPosition">
        <rdfs:domain rdf:resource="https://w3id.org/digitalconstruction/0.5/Entities#GeodeticBoundingBox"/>
        <rdfs:range rdf:resource="https://w3id.org/digitalconstruction/0.5/Entities#GeodeticPosition"/>
        <rdfs:label>hasMaximumGeodeticPosition</rdfs:label>
    </owl:ObjectProperty>
    


    <!-- https://w3id.org/digitalconstruction/0.5/Entities#hasMember -->

    <owl:ObjectProperty rdf:about="https://w3id.org/digitalconstruction/0.5/Entities#hasMember">
        <rdfs:subPropertyOf rdf:resource="http://www.w3.org/2002/07/owl#topObjectProperty"/>
        <owl:inverseOf rdf:resource="https://w3id.org/digitalconstruction/0.5/Entities#memberOf"/>
        <rdfs:domain rdf:resource="https://w3id.org/digitalconstruction/0.5/Entities#Group"/>
        <rdfs:range rdf:resource="https://w3id.org/digitalconstruction/0.5/Entities#Entity"/>
        <rdfs:label>hasMember</rdfs:label>
    </owl:ObjectProperty>
    


    <!-- https://w3id.org/digitalconstruction/0.5/Entities#hasMemberPart -->

    <owl:ObjectProperty rdf:about="https://w3id.org/digitalconstruction/0.5/Entities#hasMemberPart">
        <rdfs:subPropertyOf rdf:resource="https://w3id.org/digitalconstruction/0.5/Entities#hasContinuantPart"/>
        <owl:inverseOf rdf:resource="https://w3id.org/digitalconstruction/0.5/Entities#isMemberPartOf"/>
        <rdfs:domain rdf:resource="https://w3id.org/digitalconstruction/0.5/Entities#MaterialEntity"/>
        <rdfs:range rdf:resource="https://w3id.org/digitalconstruction/0.5/Entities#MaterialEntity"/>
        <rdfs:comment>hasMemberPart is equivalent to the BFO property &apos;has member part at some time&apos; (http://purl.obolibrary.org/obo/BFO_0000115)</rdfs:comment>
        <rdfs:label>hasMemberPart</rdfs:label>
    </owl:ObjectProperty>
    


    <!-- https://w3id.org/digitalconstruction/0.5/Entities#hasMemberPartAtAllTimes -->

    <owl:ObjectProperty rdf:about="https://w3id.org/digitalconstruction/0.5/Entities#hasMemberPartAtAllTimes">
        <rdfs:subPropertyOf rdf:resource="https://w3id.org/digitalconstruction/0.5/Entities#hasContinuantPartAtAllTimes"/>
        <rdfs:subPropertyOf rdf:resource="https://w3id.org/digitalconstruction/0.5/Entities#hasMemberPart"/>
        <rdfs:domain rdf:resource="https://w3id.org/digitalconstruction/0.5/Entities#MaterialEntity"/>
        <rdfs:range rdf:resource="https://w3id.org/digitalconstruction/0.5/Entities#MaterialEntity"/>
        <rdfs:comment>hasMemberPartAtAllTimes is equivalent to the BFO property &apos;has member part at all times&apos; (http://purl.obolibrary.org/obo/BFO_0000172)</rdfs:comment>
        <rdfs:label>hasMemberPartAtAllTimes</rdfs:label>
    </owl:ObjectProperty>
    


    <!-- https://w3id.org/digitalconstruction/0.5/Entities#hasMinimumCartesianPosition -->

    <owl:ObjectProperty rdf:about="https://w3id.org/digitalconstruction/0.5/Entities#hasMinimumCartesianPosition">
        <rdfs:domain rdf:resource="https://w3id.org/digitalconstruction/0.5/Entities#CartesianBoundingBox"/>
        <rdfs:range rdf:resource="https://w3id.org/digitalconstruction/0.5/Entities#CartesianPosition"/>
        <rdfs:label>hasMinumumCartesianPosition</rdfs:label>
    </owl:ObjectProperty>
    


    <!-- https://w3id.org/digitalconstruction/0.5/Entities#hasMinimumGeodeticPosition -->

    <owl:ObjectProperty rdf:about="https://w3id.org/digitalconstruction/0.5/Entities#hasMinimumGeodeticPosition">
        <rdfs:domain rdf:resource="https://w3id.org/digitalconstruction/0.5/Entities#GeodeticBoundingBox"/>
        <rdfs:range rdf:resource="https://w3id.org/digitalconstruction/0.5/Entities#GeodeticPosition"/>
        <rdfs:label>hasMinimumGeodeticPosition</rdfs:label>
    </owl:ObjectProperty>
    


    <!-- https://w3id.org/digitalconstruction/0.5/Entities#hasOccurrentPart -->

    <owl:ObjectProperty rdf:about="https://w3id.org/digitalconstruction/0.5/Entities#hasOccurrentPart">
        <rdfs:subPropertyOf rdf:resource="https://w3id.org/digitalconstruction/0.5/Entities#hasPart"/>
        <rdf:type rdf:resource="http://www.w3.org/2002/07/owl#TransitiveProperty"/>
        <rdfs:domain rdf:resource="https://w3id.org/digitalconstruction/0.5/Entities#Occurrent"/>
        <rdfs:range rdf:resource="https://w3id.org/digitalconstruction/0.5/Entities#Occurrent"/>
        <rdfs:comment>hasOccurrentPart is equivalent to the BFO property &apos;has occurrent part&apos; (http://purl.obolibrary.org/obo/BFO_0000117)</rdfs:comment>
        <rdfs:label>hasOccurrentPart</rdfs:label>
    </owl:ObjectProperty>
    


    <!-- https://w3id.org/digitalconstruction/0.5/Entities#hasPart -->

    <owl:ObjectProperty rdf:about="https://w3id.org/digitalconstruction/0.5/Entities#hasPart">
        <rdfs:subPropertyOf rdf:resource="http://www.w3.org/2002/07/owl#topObjectProperty"/>
        <owl:inverseOf rdf:resource="https://w3id.org/digitalconstruction/0.5/Entities#isPartOf"/>
        <rdfs:domain rdf:resource="https://w3id.org/digitalconstruction/0.5/Entities#Entity"/>
        <rdfs:range rdf:resource="https://w3id.org/digitalconstruction/0.5/Entities#Entity"/>
        <rdfs:label>hasPart</rdfs:label>
    </owl:ObjectProperty>
    


    <!-- https://w3id.org/digitalconstruction/0.5/Entities#hasParticipant -->

    <owl:ObjectProperty rdf:about="https://w3id.org/digitalconstruction/0.5/Entities#hasParticipant">
        <owl:inverseOf rdf:resource="https://w3id.org/digitalconstruction/0.5/Entities#participatesIn"/>
        <rdfs:domain rdf:resource="https://w3id.org/digitalconstruction/0.5/Entities#Process"/>
        <rdfs:range>
            <owl:Class>
                <owl:unionOf rdf:parseType="Collection">
                    <rdf:Description rdf:about="https://w3id.org/digitalconstruction/0.5/Entities#GenericallyDependentContinuant"/>
                    <rdf:Description rdf:about="https://w3id.org/digitalconstruction/0.5/Entities#SpecificallyDependentContinuant"/>
                    <owl:Class>
                        <owl:intersectionOf rdf:parseType="Collection">
                            <rdf:Description rdf:about="https://w3id.org/digitalconstruction/0.5/Entities#IndependentContinuant"/>
                            <owl:Class>
                                <owl:complementOf rdf:resource="https://w3id.org/digitalconstruction/0.5/Entities#SpatialRegion"/>
                            </owl:Class>
                        </owl:intersectionOf>
                    </owl:Class>
                </owl:unionOf>
            </owl:Class>
        </rdfs:range>
        <rdfs:comment>hasParticipant is equivalent to the BFO property &apos;has participant at some time&apos; (http://purl.obolibrary.org/obo/BFO_0000057)</rdfs:comment>
        <rdfs:label>hasParticipant</rdfs:label>
    </owl:ObjectProperty>
    


    <!-- https://w3id.org/digitalconstruction/0.5/Entities#hasParticipantAtAllTimes -->

    <owl:ObjectProperty rdf:about="https://w3id.org/digitalconstruction/0.5/Entities#hasParticipantAtAllTimes">
        <rdfs:subPropertyOf rdf:resource="https://w3id.org/digitalconstruction/0.5/Entities#hasParticipant"/>
        <rdfs:domain rdf:resource="https://w3id.org/digitalconstruction/0.5/Entities#Process"/>
        <rdfs:range>
            <owl:Class>
                <owl:unionOf rdf:parseType="Collection">
                    <rdf:Description rdf:about="https://w3id.org/digitalconstruction/0.5/Entities#GenericallyDependentContinuant"/>
                    <rdf:Description rdf:about="https://w3id.org/digitalconstruction/0.5/Entities#SpecificallyDependentContinuant"/>
                    <owl:Class>
                        <owl:intersectionOf rdf:parseType="Collection">
                            <rdf:Description rdf:about="https://w3id.org/digitalconstruction/0.5/Entities#IndependentContinuant"/>
                            <owl:Class>
                                <owl:complementOf rdf:resource="https://w3id.org/digitalconstruction/0.5/Entities#SpatialRegion"/>
                            </owl:Class>
                        </owl:intersectionOf>
                    </owl:Class>
                </owl:unionOf>
            </owl:Class>
        </rdfs:range>
        <rdfs:comment>hasParticipantAtAllTimes is equivalent to the BFO property &apos;has participant at all times&apos; (http://purl.obolibrary.org/obo/BFO_0000167)</rdfs:comment>
        <rdfs:label>hasParticipantAtAllTimes</rdfs:label>
    </owl:ObjectProperty>
    


    <!-- https://w3id.org/digitalconstruction/0.5/Entities#hasProperContinuantPart -->

    <owl:ObjectProperty rdf:about="https://w3id.org/digitalconstruction/0.5/Entities#hasProperContinuantPart">
        <rdfs:subPropertyOf rdf:resource="https://w3id.org/digitalconstruction/0.5/Entities#hasContinuantPart"/>
        <rdfs:domain rdf:resource="https://w3id.org/digitalconstruction/0.5/Entities#Continuant"/>
        <rdfs:range rdf:resource="https://w3id.org/digitalconstruction/0.5/Entities#Continuant"/>
        <rdfs:comment>hasProperContinuantPart is equivalent to the BFO property &apos;has proper continuant part at some time&apos; (http://purl.obolibrary.org/obo/BFO_0000174)</rdfs:comment>
        <rdfs:label>hasProperContinuantPart</rdfs:label>
    </owl:ObjectProperty>
    


    <!-- https://w3id.org/digitalconstruction/0.5/Entities#hasProperContinuantPartAtAllTimes -->

    <owl:ObjectProperty rdf:about="https://w3id.org/digitalconstruction/0.5/Entities#hasProperContinuantPartAtAllTimes">
        <rdfs:subPropertyOf rdf:resource="https://w3id.org/digitalconstruction/0.5/Entities#hasContinuantPartAtAllTimes"/>
        <rdfs:subPropertyOf rdf:resource="https://w3id.org/digitalconstruction/0.5/Entities#hasProperContinuantPart"/>
        <rdf:type rdf:resource="http://www.w3.org/2002/07/owl#TransitiveProperty"/>
        <rdfs:domain rdf:resource="https://w3id.org/digitalconstruction/0.5/Entities#Continuant"/>
        <rdfs:range rdf:resource="https://w3id.org/digitalconstruction/0.5/Entities#Continuant"/>
        <rdfs:comment>hasProperContinuantPartAtAllTimes is equivalent to the BFO property &apos;has proper continuant part at all times&apos; (http://purl.obolibrary.org/obo/BFO_0000111)</rdfs:comment>
        <rdfs:label>hasProperContinuantPartAtAllTimes</rdfs:label>
    </owl:ObjectProperty>
    


    <!-- https://w3id.org/digitalconstruction/0.5/Entities#hasProperOccurrentPart -->

    <owl:ObjectProperty rdf:about="https://w3id.org/digitalconstruction/0.5/Entities#hasProperOccurrentPart">
        <rdfs:subPropertyOf rdf:resource="https://w3id.org/digitalconstruction/0.5/Entities#hasOccurrentPart"/>
        <rdfs:domain rdf:resource="https://w3id.org/digitalconstruction/0.5/Entities#Occurrent"/>
        <rdfs:range rdf:resource="https://w3id.org/digitalconstruction/0.5/Entities#Occurrent"/>
        <rdfs:comment>hasProperOccurrentPart is equivalent to the BFO property &apos;has proper occurrent part&apos; (http://purl.obolibrary.org/obo/BFO_0000118)</rdfs:comment>
        <rdfs:label>hasProperOccurrentPart</rdfs:label>
    </owl:ObjectProperty>
    


    <!-- https://w3id.org/digitalconstruction/0.5/Entities#hasProperTemporalPart -->

    <owl:ObjectProperty rdf:about="https://w3id.org/digitalconstruction/0.5/Entities#hasProperTemporalPart">
        <rdfs:subPropertyOf rdf:resource="https://w3id.org/digitalconstruction/0.5/Entities#hasTemporalPart"/>
        <rdfs:domain rdf:resource="https://w3id.org/digitalconstruction/0.5/Entities#Occurrent"/>
        <rdfs:range rdf:resource="https://w3id.org/digitalconstruction/0.5/Entities#Occurrent"/>
        <rdfs:comment>hasProperTemporalPart is equivalent to the BFO property &apos;has proper temporal part&apos; (http://purl.obolibrary.org/obo/BFO_0000181)</rdfs:comment>
        <rdfs:label>hasProperTemporalPart</rdfs:label>
    </owl:ObjectProperty>
    


    <!-- https://w3id.org/digitalconstruction/0.5/Entities#hasQuality -->

    <owl:ObjectProperty rdf:about="https://w3id.org/digitalconstruction/0.5/Entities#hasQuality">
        <rdfs:subPropertyOf rdf:resource="https://w3id.org/digitalconstruction/0.5/Entities#bearerOf"/>
        <owl:inverseOf rdf:resource="https://w3id.org/digitalconstruction/0.5/Entities#isQualityOf"/>
        <rdfs:range rdf:resource="https://w3id.org/digitalconstruction/0.5/Entities#Quality"/>
        <rdfs:label>hasQuality</rdfs:label>
    </owl:ObjectProperty>
    


    <!-- https://w3id.org/digitalconstruction/0.5/Entities#hasRealization -->

    <owl:ObjectProperty rdf:about="https://w3id.org/digitalconstruction/0.5/Entities#hasRealization">
        <rdfs:domain rdf:resource="https://w3id.org/digitalconstruction/0.5/Entities#RealizableEntity"/>
        <rdfs:range rdf:resource="https://w3id.org/digitalconstruction/0.5/Entities#Process"/>
        <rdfs:comment>hasRealization is equivalent to the BFO property &apos;has realization&apos; (http://purl.obolibrary.org/obo/BFO_0000054)</rdfs:comment>
        <rdfs:label>hasRealization</rdfs:label>
    </owl:ObjectProperty>
    


    <!-- https://w3id.org/digitalconstruction/0.5/Entities#hasRole -->

    <owl:ObjectProperty rdf:about="https://w3id.org/digitalconstruction/0.5/Entities#hasRole">
        <owl:inverseOf rdf:resource="https://w3id.org/digitalconstruction/0.5/Entities#isRoleOf"/>
        <rdfs:range rdf:resource="https://w3id.org/digitalconstruction/0.5/Entities#Role"/>
        <rdfs:label>hasRole</rdfs:label>
    </owl:ObjectProperty>
    


    <!-- https://w3id.org/digitalconstruction/0.5/Entities#hasScope -->

    <owl:ObjectProperty rdf:about="https://w3id.org/digitalconstruction/0.5/Entities#hasScope">
        <rdfs:domain rdf:resource="https://w3id.org/digitalconstruction/0.5/Entities#Labeling"/>
        <rdfs:range rdf:resource="https://w3id.org/digitalconstruction/0.5/Entities#Category"/>
        <rdfs:comment>Defines the broader category that is the scope of the label</rdfs:comment>
        <rdfs:label>hasScope</rdfs:label>
    </owl:ObjectProperty>
    


    <!-- https://w3id.org/digitalconstruction/0.5/Entities#hasSpatialExtent -->

    <owl:ObjectProperty rdf:about="https://w3id.org/digitalconstruction/0.5/Entities#hasSpatialExtent">
        <rdfs:domain rdf:resource="https://w3id.org/digitalconstruction/0.5/Entities#SpatialRegion"/>
        <rdfs:range rdf:resource="https://w3id.org/digitalconstruction/0.5/Entities#SpatialExtent"/>
        <rdfs:label>hasSpatialExtent</rdfs:label>
    </owl:ObjectProperty>
    


    <!-- https://w3id.org/digitalconstruction/0.5/Entities#hasSpatialOrientation -->

    <owl:ObjectProperty rdf:about="https://w3id.org/digitalconstruction/0.5/Entities#hasSpatialOrientation">
        <rdfs:domain rdf:resource="https://w3id.org/digitalconstruction/0.5/Entities#CartesianPosition"/>
        <rdfs:range rdf:resource="https://w3id.org/digitalconstruction/0.5/Entities#SpatialOrientation"/>
        <rdfs:label>hasSpatialOrientation</rdfs:label>
    </owl:ObjectProperty>
    


    <!-- https://w3id.org/digitalconstruction/0.5/Entities#hasSpatialOrigin -->

    <owl:ObjectProperty rdf:about="https://w3id.org/digitalconstruction/0.5/Entities#hasSpatialOrigin">
        <rdfs:domain rdf:resource="https://w3id.org/digitalconstruction/0.5/Entities#CartesianPosition"/>
        <rdfs:range rdf:resource="https://w3id.org/digitalconstruction/0.5/Entities#SpatialPosition"/>
        <rdfs:label>hasSpatialOrigin</rdfs:label>
    </owl:ObjectProperty>
    


    <!-- https://w3id.org/digitalconstruction/0.5/Entities#hasSpatialPosition -->

    <owl:ObjectProperty rdf:about="https://w3id.org/digitalconstruction/0.5/Entities#hasSpatialPosition">
        <rdfs:domain rdf:resource="https://w3id.org/digitalconstruction/0.5/Entities#SpatialRegion"/>
        <rdfs:range rdf:resource="https://w3id.org/digitalconstruction/0.5/Entities#SpatialPosition"/>
        <rdfs:label>hasSpatialPosition</rdfs:label>
    </owl:ObjectProperty>
    


    <!-- https://w3id.org/digitalconstruction/0.5/Entities#hasStart -->

    <owl:ObjectProperty rdf:about="https://w3id.org/digitalconstruction/0.5/Entities#hasStart">
        <rdfs:subPropertyOf rdf:resource="https://w3id.org/digitalconstruction/0.5/Entities#hasFirstInstant"/>
        <owl:inverseOf rdf:resource="https://w3id.org/digitalconstruction/0.5/Entities#isStartOf"/>
        <rdfs:domain rdf:resource="https://w3id.org/digitalconstruction/0.5/Entities#TimeInterval"/>
        <rdfs:range rdf:resource="https://w3id.org/digitalconstruction/0.5/Entities#TimeInstant"/>
        <rdfs:label>hasStart</rdfs:label>
    </owl:ObjectProperty>
    


    <!-- https://w3id.org/digitalconstruction/0.5/Entities#hasSubGroup -->

    <owl:ObjectProperty rdf:about="https://w3id.org/digitalconstruction/0.5/Entities#hasSubGroup">
        <owl:inverseOf rdf:resource="https://w3id.org/digitalconstruction/0.5/Entities#isSubGroupOf"/>
        <rdfs:domain rdf:resource="https://w3id.org/digitalconstruction/0.5/Entities#Group"/>
        <rdfs:range rdf:resource="https://w3id.org/digitalconstruction/0.5/Entities#Group"/>
        <rdfs:label>hasSubGroup</rdfs:label>
    </owl:ObjectProperty>
    


    <!-- https://w3id.org/digitalconstruction/0.5/Entities#hasSubLocation -->

    <owl:ObjectProperty rdf:about="https://w3id.org/digitalconstruction/0.5/Entities#hasSubLocation">
        <rdfs:subPropertyOf rdf:resource="https://w3id.org/digitalconstruction/0.5/Entities#hasLocationAtAllTimes"/>
        <owl:inverseOf rdf:resource="https://w3id.org/digitalconstruction/0.5/Entities#isSubLocationOf"/>
        <rdfs:domain rdf:resource="https://w3id.org/digitalconstruction/0.5/Entities#Location"/>
        <rdfs:range rdf:resource="https://w3id.org/digitalconstruction/0.5/Entities#Location"/>
        <rdfs:label>hasSubLocation</rdfs:label>
    </owl:ObjectProperty>
    


    <!-- https://w3id.org/digitalconstruction/0.5/Entities#hasTemporalPart -->

    <owl:ObjectProperty rdf:about="https://w3id.org/digitalconstruction/0.5/Entities#hasTemporalPart">
        <rdfs:subPropertyOf rdf:resource="https://w3id.org/digitalconstruction/0.5/Entities#hasOccurrentPart"/>
        <rdf:type rdf:resource="http://www.w3.org/2002/07/owl#TransitiveProperty"/>
        <rdfs:domain rdf:resource="https://w3id.org/digitalconstruction/0.5/Entities#Occurrent"/>
        <rdfs:range rdf:resource="https://w3id.org/digitalconstruction/0.5/Entities#Occurrent"/>
        <rdfs:comment>hasTemporalPart is equivalent to the BFO property &apos;has temporal part&apos; (http://purl.obolibrary.org/obo/BFO_0000121)</rdfs:comment>
        <rdfs:label>hasTemporalPart</rdfs:label>
    </owl:ObjectProperty>
    


    <!-- https://w3id.org/digitalconstruction/0.5/Entities#historyOf -->

    <owl:ObjectProperty rdf:about="https://w3id.org/digitalconstruction/0.5/Entities#historyOf">
        <rdf:type rdf:resource="http://www.w3.org/2002/07/owl#FunctionalProperty"/>
        <rdf:type rdf:resource="http://www.w3.org/2002/07/owl#InverseFunctionalProperty"/>
        <rdfs:domain rdf:resource="https://w3id.org/digitalconstruction/0.5/Entities#History"/>
        <rdfs:range rdf:resource="https://w3id.org/digitalconstruction/0.5/Entities#MaterialEntity"/>
        <rdfs:comment>historyOf is equivalent to the BFO property &apos;history of&apos; (http://purl.obolibrary.org/obo/BFO_0000184)</rdfs:comment>
        <rdfs:label>historyOf</rdfs:label>
    </owl:ObjectProperty>
    


    <!-- https://w3id.org/digitalconstruction/0.5/Entities#identifies -->

    <owl:ObjectProperty rdf:about="https://w3id.org/digitalconstruction/0.5/Entities#identifies">
        <rdfs:subPropertyOf rdf:resource="https://w3id.org/digitalconstruction/0.5/Entities#labels"/>
        <owl:inverseOf rdf:resource="https://w3id.org/digitalconstruction/0.5/Entities#isIdentifiedBy"/>
        <rdfs:domain rdf:resource="https://w3id.org/digitalconstruction/0.5/Entities#Identifier"/>
        <rdfs:range rdf:resource="https://w3id.org/digitalconstruction/0.5/Entities#Entity"/>
        <rdfs:label>identifies</rdfs:label>
    </owl:ObjectProperty>
    


    <!-- https://w3id.org/digitalconstruction/0.5/Entities#includesRole -->

    <owl:ObjectProperty rdf:about="https://w3id.org/digitalconstruction/0.5/Entities#includesRole">
        <owl:inverseOf rdf:resource="https://w3id.org/digitalconstruction/0.5/Entities#isIncludedRoleIn"/>
        <rdfs:domain rdf:resource="https://w3id.org/digitalconstruction/0.5/Entities#Entity"/>
        <rdfs:range rdf:resource="https://w3id.org/digitalconstruction/0.5/Entities#Role"/>
        <rdfs:label>includesRole</rdfs:label>
    </owl:ObjectProperty>
    


    <!-- https://w3id.org/digitalconstruction/0.5/Entities#inheresIn -->

    <owl:ObjectProperty rdf:about="https://w3id.org/digitalconstruction/0.5/Entities#inheresIn">
        <rdfs:subPropertyOf rdf:resource="https://w3id.org/digitalconstruction/0.5/Entities#specificallyDependsOn"/>
        <rdfs:domain rdf:resource="https://w3id.org/digitalconstruction/0.5/Entities#SpecificallyDependentContinuant"/>
        <rdfs:range>
            <owl:Class>
                <owl:intersectionOf rdf:parseType="Collection">
                    <rdf:Description rdf:about="https://w3id.org/digitalconstruction/0.5/Entities#IndependentContinuant"/>
                    <owl:Class>
                        <owl:complementOf rdf:resource="https://w3id.org/digitalconstruction/0.5/Entities#SpatialRegion"/>
                    </owl:Class>
                </owl:intersectionOf>
            </owl:Class>
        </rdfs:range>
        <rdfs:comment>inheresIn is equivalent to the BFO property &apos;inheres in&apos; (http://purl.obolibrary.org/obo/BFO_0000197)</rdfs:comment>
        <rdfs:label>inheresIn</rdfs:label>
    </owl:ObjectProperty>
    


    <!-- https://w3id.org/digitalconstruction/0.5/Entities#isAssignedToInstance -->

    <owl:ObjectProperty rdf:about="https://w3id.org/digitalconstruction/0.5/Entities#isAssignedToInstance">
        <rdfs:subPropertyOf rdf:resource="https://w3id.org/digitalconstruction/0.5/Entities#isIdentifiedBy"/>
        <rdfs:domain rdf:resource="https://w3id.org/digitalconstruction/0.5/Entities#MaterialEntity"/>
        <rdfs:range rdf:resource="https://w3id.org/digitalconstruction/0.5/Entities#Identifier"/>
        <rdfs:label>isAssignedToInstance</rdfs:label>
    </owl:ObjectProperty>
    


    <!-- https://w3id.org/digitalconstruction/0.5/Entities#isAssignedToType -->

    <owl:ObjectProperty rdf:about="https://w3id.org/digitalconstruction/0.5/Entities#isAssignedToType">
        <rdfs:subPropertyOf rdf:resource="https://w3id.org/digitalconstruction/0.5/Entities#isClassifiedBy"/>
        <rdfs:domain rdf:resource="https://w3id.org/digitalconstruction/0.5/Entities#MaterialEntity"/>
        <rdfs:range rdf:resource="https://w3id.org/digitalconstruction/0.5/Entities#Category"/>
        <rdfs:comment>Assigns a selected type to an entity. The classification is not descriptive but rather a restriction to some subtype of the original type. An example is product assignment.</rdfs:comment>
        <rdfs:label>isAssignedToType</rdfs:label>
    </owl:ObjectProperty>
    


    <!-- https://w3id.org/digitalconstruction/0.5/Entities#isBuildingOf -->

    <owl:ObjectProperty rdf:about="https://w3id.org/digitalconstruction/0.5/Entities#isBuildingOf">
        <rdfs:domain rdf:resource="https://w3id.org/digitalconstruction/0.5/Entities#Building"/>
        <rdfs:range rdf:resource="https://w3id.org/digitalconstruction/0.5/Entities#RealEstate"/>
    </owl:ObjectProperty>
    


    <!-- https://w3id.org/digitalconstruction/0.5/Entities#isBuildingUnitOf -->

    <owl:ObjectProperty rdf:about="https://w3id.org/digitalconstruction/0.5/Entities#isBuildingUnitOf">
        <rdfs:domain rdf:resource="https://w3id.org/digitalconstruction/0.5/Entities#BuildingUnit"/>
        <rdfs:range rdf:resource="https://w3id.org/digitalconstruction/0.5/Entities#Building"/>
    </owl:ObjectProperty>
    


    <!-- https://w3id.org/digitalconstruction/0.5/Entities#isCapabilityOf -->

    <owl:ObjectProperty rdf:about="https://w3id.org/digitalconstruction/0.5/Entities#isCapabilityOf">
        <rdfs:subPropertyOf rdf:resource="https://w3id.org/digitalconstruction/0.5/Entities#inheresIn"/>
        <rdfs:domain rdf:resource="https://w3id.org/digitalconstruction/0.5/Entities#Capability"/>
        <rdfs:range rdf:resource="https://w3id.org/digitalconstruction/0.5/Entities#MaterialEntity"/>
        <rdfs:label>isCapabilityOf</rdfs:label>
    </owl:ObjectProperty>
    


    <!-- https://w3id.org/digitalconstruction/0.5/Entities#isCarrierOf -->

    <owl:ObjectProperty rdf:about="https://w3id.org/digitalconstruction/0.5/Entities#isCarrierOf">
        <rdfs:domain>
            <owl:Class>
                <owl:intersectionOf rdf:parseType="Collection">
                    <rdf:Description rdf:about="https://w3id.org/digitalconstruction/0.5/Entities#IndependentContinuant"/>
                    <owl:Class>
                        <owl:complementOf rdf:resource="https://w3id.org/digitalconstruction/0.5/Entities#SpatialRegion"/>
                    </owl:Class>
                </owl:intersectionOf>
            </owl:Class>
        </rdfs:domain>
        <rdfs:range rdf:resource="https://w3id.org/digitalconstruction/0.5/Entities#GenericallyDependentContinuant"/>
        <rdfs:comment>isCarrierOf is equivalent to the BFO property &apos;is carrier of at some time&apos; (http://purl.obolibrary.org/obo/BFO_0000101)</rdfs:comment>
        <rdfs:label>isCarrierOf</rdfs:label>
    </owl:ObjectProperty>
    


    <!-- https://w3id.org/digitalconstruction/0.5/Entities#isCarrierOfAtAllTimes -->

    <owl:ObjectProperty rdf:about="https://w3id.org/digitalconstruction/0.5/Entities#isCarrierOfAtAllTimes">
        <rdfs:subPropertyOf rdf:resource="https://w3id.org/digitalconstruction/0.5/Entities#isCarrierOf"/>
        <rdfs:domain>
            <owl:Class>
                <owl:intersectionOf rdf:parseType="Collection">
                    <rdf:Description rdf:about="https://w3id.org/digitalconstruction/0.5/Entities#IndependentContinuant"/>
                    <owl:Class>
                        <owl:complementOf rdf:resource="https://w3id.org/digitalconstruction/0.5/Entities#SpatialRegion"/>
                    </owl:Class>
                </owl:intersectionOf>
            </owl:Class>
        </rdfs:domain>
        <rdfs:range rdf:resource="https://w3id.org/digitalconstruction/0.5/Entities#GenericallyDependentContinuant"/>
        <rdfs:comment>isCarrierOfAtAllTimes is equivalent to the BFO property &apos;is carrier of at all times&apos; (http://purl.obolibrary.org/obo/BFO_0000220)</rdfs:comment>
        <rdfs:label>isCarrierOfAtAllTimes</rdfs:label>
    </owl:ObjectProperty>
    


    <!-- https://w3id.org/digitalconstruction/0.5/Entities#isClassifiedBy -->

    <owl:ObjectProperty rdf:about="https://w3id.org/digitalconstruction/0.5/Entities#isClassifiedBy">
        <rdfs:subPropertyOf rdf:resource="https://w3id.org/digitalconstruction/0.5/Entities#labeledBy"/>
        <rdfs:domain rdf:resource="https://w3id.org/digitalconstruction/0.5/Entities#Entity"/>
        <rdfs:range rdf:resource="https://w3id.org/digitalconstruction/0.5/Entities#Category"/>
        <rdfs:label>isClassifiedBy</rdfs:label>
    </owl:ObjectProperty>
    


    <!-- https://w3id.org/digitalconstruction/0.5/Entities#isConcretizedBy -->

    <owl:ObjectProperty rdf:about="https://w3id.org/digitalconstruction/0.5/Entities#isConcretizedBy">
        <rdfs:domain rdf:resource="https://w3id.org/digitalconstruction/0.5/Entities#GenericallyDependentContinuant"/>
        <rdfs:range>
            <owl:Class>
                <owl:unionOf rdf:parseType="Collection">
                    <rdf:Description rdf:about="https://w3id.org/digitalconstruction/0.5/Entities#Process"/>
                    <rdf:Description rdf:about="https://w3id.org/digitalconstruction/0.5/Entities#SpecificallyDependentContinuant"/>
                </owl:unionOf>
            </owl:Class>
        </rdfs:range>
        <rdfs:comment>isConcretizedBy is equivalent to the BFO property &apos;is concretized by at some time&apos; (http://purl.obolibrary.org/obo/BFO_0000058)</rdfs:comment>
        <rdfs:label>isConcretizedBy</rdfs:label>
    </owl:ObjectProperty>
    


    <!-- https://w3id.org/digitalconstruction/0.5/Entities#isConcretizedByAtAllTimes -->

    <owl:ObjectProperty rdf:about="https://w3id.org/digitalconstruction/0.5/Entities#isConcretizedByAtAllTimes">
        <rdfs:subPropertyOf rdf:resource="https://w3id.org/digitalconstruction/0.5/Entities#isConcretizedBy"/>
        <rdfs:domain rdf:resource="https://w3id.org/digitalconstruction/0.5/Entities#GenericallyDependentContinuant"/>
        <rdfs:range>
            <owl:Class>
                <owl:unionOf rdf:parseType="Collection">
                    <rdf:Description rdf:about="https://w3id.org/digitalconstruction/0.5/Entities#Process"/>
                    <rdf:Description rdf:about="https://w3id.org/digitalconstruction/0.5/Entities#SpecificallyDependentContinuant"/>
                </owl:unionOf>
            </owl:Class>
        </rdfs:range>
        <rdfs:comment>isConcretizedByAtAllTimes is equivalent to the BFO property &apos;is concretized by at all times&apos; (http://purl.obolibrary.org/obo/BFO_0000165)</rdfs:comment>
        <rdfs:label>isConcretizedByAtAllTimes</rdfs:label>
    </owl:ObjectProperty>
    


    <!-- https://w3id.org/digitalconstruction/0.5/Entities#isDeterminedBy -->

    <owl:ObjectProperty rdf:about="https://w3id.org/digitalconstruction/0.5/Entities#isDeterminedBy">
        <rdfs:domain rdf:resource="https://w3id.org/digitalconstruction/0.5/Variables#PropertyState"/>
        <rdfs:range rdf:resource="https://w3id.org/digitalconstruction/0.5/Entities#MaterialEntity"/>
        <rdfs:comment>The material entity that has determined the value of the property state. For example, an agent or a sensor</rdfs:comment>
        <rdfs:label>isDeterminedBy</rdfs:label>
    </owl:ObjectProperty>
    


    <!-- https://w3id.org/digitalconstruction/0.5/Entities#isEndOf -->

    <owl:ObjectProperty rdf:about="https://w3id.org/digitalconstruction/0.5/Entities#isEndOf">
        <rdfs:subPropertyOf rdf:resource="https://w3id.org/digitalconstruction/0.5/Entities#hasFirstInstant"/>
        <rdfs:domain rdf:resource="https://w3id.org/digitalconstruction/0.5/Entities#TimeInstant"/>
        <rdfs:range rdf:resource="https://w3id.org/digitalconstruction/0.5/Entities#TimeInterval"/>
        <rdfs:label>isEndOf</rdfs:label>
    </owl:ObjectProperty>
    


    <!-- https://w3id.org/digitalconstruction/0.5/Entities#isEntityStateOf -->

    <owl:ObjectProperty rdf:about="https://w3id.org/digitalconstruction/0.5/Entities#isEntityStateOf">
        <rdfs:domain rdf:resource="https://w3id.org/digitalconstruction/0.5/Entities#EntityState"/>
        <rdfs:range rdf:resource="https://w3id.org/digitalconstruction/0.5/Entities#Entity"/>
        <rdfs:comment>Entity that the state applies to</rdfs:comment>
        <rdfs:label>isEntityStateOf</rdfs:label>
    </owl:ObjectProperty>
    


    <!-- https://w3id.org/digitalconstruction/0.5/Entities#isEnvironmentOf -->

    <owl:ObjectProperty rdf:about="https://w3id.org/digitalconstruction/0.5/Entities#isEnvironmentOf">
        <owl:inverseOf rdf:resource="https://w3id.org/digitalconstruction/0.5/Entities#occursIn"/>
        <rdfs:label>isEnvironmentOf</rdfs:label>
    </owl:ObjectProperty>
    


    <!-- https://w3id.org/digitalconstruction/0.5/Entities#isEquipmentIn -->

    <owl:ObjectProperty rdf:about="https://w3id.org/digitalconstruction/0.5/Entities#isEquipmentIn">
        <rdfs:subPropertyOf rdf:resource="https://w3id.org/digitalconstruction/0.5/Entities#participatesIn"/>
        <rdfs:domain rdf:resource="https://w3id.org/digitalconstruction/0.5/Entities#Equipment"/>
        <rdfs:range rdf:resource="https://w3id.org/digitalconstruction/0.5/Entities#Process"/>
        <rdfs:label>isEquipmentIn</rdfs:label>
    </owl:ObjectProperty>
    


    <!-- https://w3id.org/digitalconstruction/0.5/Entities#isIdentifiedBy -->

    <owl:ObjectProperty rdf:about="https://w3id.org/digitalconstruction/0.5/Entities#isIdentifiedBy">
        <rdfs:subPropertyOf rdf:resource="https://w3id.org/digitalconstruction/0.5/Entities#labeledBy"/>
        <rdfs:domain rdf:resource="https://w3id.org/digitalconstruction/0.5/Entities#Entity"/>
        <rdfs:range rdf:resource="https://w3id.org/digitalconstruction/0.5/Entities#Identifier"/>
        <rdfs:label>isIdentifiedBy</rdfs:label>
    </owl:ObjectProperty>
    


    <!-- https://w3id.org/digitalconstruction/0.5/Entities#isIncludedRoleIn -->

    <owl:ObjectProperty rdf:about="https://w3id.org/digitalconstruction/0.5/Entities#isIncludedRoleIn">
        <rdfs:domain rdf:resource="https://w3id.org/digitalconstruction/0.5/Entities#Role"/>
        <rdfs:range rdf:resource="https://w3id.org/digitalconstruction/0.5/Entities#Entity"/>
        <rdfs:label>isIncludedRoleIn</rdfs:label>
    </owl:ObjectProperty>
    


    <!-- https://w3id.org/digitalconstruction/0.5/Entities#isLabeledBy -->

    <owl:ObjectProperty rdf:about="https://w3id.org/digitalconstruction/0.5/Entities#isLabeledBy">
        <rdfs:subPropertyOf rdf:resource="https://w3id.org/digitalconstruction/0.5/Variables#hasProperty"/>
        <owl:inverseOf rdf:resource="https://w3id.org/digitalconstruction/0.5/Entities#labels"/>
        <rdfs:domain rdf:resource="https://w3id.org/digitalconstruction/0.5/Entities#Entity"/>
        <rdfs:range rdf:resource="https://w3id.org/digitalconstruction/0.5/Entities#Labeling"/>
        <rdfs:label>isLabeledBy</rdfs:label>
    </owl:ObjectProperty>
    


    <!-- https://w3id.org/digitalconstruction/0.5/Entities#isLocatedIn -->

    <owl:ObjectProperty rdf:about="https://w3id.org/digitalconstruction/0.5/Entities#isLocatedIn">
        <owl:inverseOf rdf:resource="https://w3id.org/digitalconstruction/0.5/Entities#isLocationOf"/>
        <rdfs:domain rdf:resource="https://w3id.org/digitalconstruction/0.5/Entities#MaterialEntity"/>
        <rdfs:range rdf:resource="https://w3id.org/digitalconstruction/0.5/Entities#Location"/>
        <rdfs:label>isLocatedIn</rdfs:label>
    </owl:ObjectProperty>
    


    <!-- https://w3id.org/digitalconstruction/0.5/Entities#isLocationOf -->

    <owl:ObjectProperty rdf:about="https://w3id.org/digitalconstruction/0.5/Entities#isLocationOf">
        <rdfs:domain rdf:resource="https://w3id.org/digitalconstruction/0.5/Entities#Location"/>
        <rdfs:range rdf:resource="https://w3id.org/digitalconstruction/0.5/Entities#MaterialEntity"/>
        <rdfs:label>isLocationOf</rdfs:label>
    </owl:ObjectProperty>
    


    <!-- https://w3id.org/digitalconstruction/0.5/Entities#isMemberPartOf -->

    <owl:ObjectProperty rdf:about="https://w3id.org/digitalconstruction/0.5/Entities#isMemberPartOf">
        <rdfs:label>isMemberPartOf</rdfs:label>
    </owl:ObjectProperty>
    


    <!-- https://w3id.org/digitalconstruction/0.5/Entities#isPartOf -->

    <owl:ObjectProperty rdf:about="https://w3id.org/digitalconstruction/0.5/Entities#isPartOf">
        <rdfs:subPropertyOf rdf:resource="http://www.w3.org/2002/07/owl#topObjectProperty"/>
        <rdfs:domain rdf:resource="https://w3id.org/digitalconstruction/0.5/Entities#Entity"/>
        <rdfs:range rdf:resource="https://w3id.org/digitalconstruction/0.5/Entities#Entity"/>
        <rdfs:label>isPartOf</rdfs:label>
    </owl:ObjectProperty>
    


    <!-- https://w3id.org/digitalconstruction/0.5/Entities#isQualityOf -->

    <owl:ObjectProperty rdf:about="https://w3id.org/digitalconstruction/0.5/Entities#isQualityOf">
        <rdfs:subPropertyOf rdf:resource="https://w3id.org/digitalconstruction/0.5/Entities#inheresIn"/>
        <rdfs:domain rdf:resource="https://w3id.org/digitalconstruction/0.5/Entities#Quality"/>
        <rdfs:label>isQualityOf</rdfs:label>
    </owl:ObjectProperty>
    


    <!-- https://w3id.org/digitalconstruction/0.5/Entities#isRoleOf -->

    <owl:ObjectProperty rdf:about="https://w3id.org/digitalconstruction/0.5/Entities#isRoleOf">
        <rdfs:subPropertyOf rdf:resource="https://w3id.org/digitalconstruction/0.5/Entities#inheresIn"/>
        <rdfs:domain rdf:resource="https://w3id.org/digitalconstruction/0.5/Entities#Role"/>
        <rdfs:label>isRoleOf</rdfs:label>
    </owl:ObjectProperty>
    


    <!-- https://w3id.org/digitalconstruction/0.5/Entities#isStartOf -->

    <owl:ObjectProperty rdf:about="https://w3id.org/digitalconstruction/0.5/Entities#isStartOf">
        <rdfs:subPropertyOf rdf:resource="https://w3id.org/digitalconstruction/0.5/Entities#firstInstantOf"/>
        <rdfs:domain rdf:resource="https://w3id.org/digitalconstruction/0.5/Entities#TimeInstant"/>
        <rdfs:range rdf:resource="https://w3id.org/digitalconstruction/0.5/Entities#TimeInterval"/>
        <rdfs:label>isStartOf</rdfs:label>
    </owl:ObjectProperty>
    


    <!-- https://w3id.org/digitalconstruction/0.5/Entities#isSubGroupOf -->

    <owl:ObjectProperty rdf:about="https://w3id.org/digitalconstruction/0.5/Entities#isSubGroupOf">
        <rdfs:domain rdf:resource="https://w3id.org/digitalconstruction/0.5/Entities#Group"/>
        <rdfs:range rdf:resource="https://w3id.org/digitalconstruction/0.5/Entities#Group"/>
        <rdfs:label>isSubGroupOf</rdfs:label>
    </owl:ObjectProperty>
    


    <!-- https://w3id.org/digitalconstruction/0.5/Entities#isSubLocationOf -->

    <owl:ObjectProperty rdf:about="https://w3id.org/digitalconstruction/0.5/Entities#isSubLocationOf">
        <rdfs:subPropertyOf rdf:resource="https://w3id.org/digitalconstruction/0.5/Entities#locatedInAtAllTimes"/>
        <rdfs:domain rdf:resource="https://w3id.org/digitalconstruction/0.5/Entities#Location"/>
        <rdfs:range rdf:resource="https://w3id.org/digitalconstruction/0.5/Entities#Location"/>
        <rdfs:label>isSubLocationOf</rdfs:label>
    </owl:ObjectProperty>
    


    <!-- https://w3id.org/digitalconstruction/0.5/Entities#labeledBy -->

    <owl:ObjectProperty rdf:about="https://w3id.org/digitalconstruction/0.5/Entities#labeledBy"/>
    


    <!-- https://w3id.org/digitalconstruction/0.5/Entities#labels -->

    <owl:ObjectProperty rdf:about="https://w3id.org/digitalconstruction/0.5/Entities#labels">
        <rdfs:subPropertyOf rdf:resource="https://w3id.org/digitalconstruction/0.5/Variables#isPropertyOf"/>
        <rdfs:domain rdf:resource="https://w3id.org/digitalconstruction/0.5/Entities#Labeling"/>
        <rdfs:range rdf:resource="https://w3id.org/digitalconstruction/0.5/Entities#Entity"/>
    </owl:ObjectProperty>
    


    <!-- https://w3id.org/digitalconstruction/0.5/Entities#lastInstantOf -->

    <owl:ObjectProperty rdf:about="https://w3id.org/digitalconstruction/0.5/Entities#lastInstantOf">
        <rdfs:domain rdf:resource="https://w3id.org/digitalconstruction/0.5/Entities#TimeInstant"/>
        <rdfs:range rdf:resource="https://w3id.org/digitalconstruction/0.5/Entities#TemporalRegion"/>
        <rdfs:comment>lastInstantOf is equivalent to the BFO property &apos;last instant of&apos; (http://purl.obolibrary.org/obo/BFO_0000223)</rdfs:comment>
        <rdfs:label>lastInstantOf</rdfs:label>
    </owl:ObjectProperty>
    


    <!-- https://w3id.org/digitalconstruction/0.5/Entities#locatedIn -->

    <owl:ObjectProperty rdf:about="https://w3id.org/digitalconstruction/0.5/Entities#locatedIn">
        <rdfs:domain>
            <owl:Class>
                <owl:intersectionOf rdf:parseType="Collection">
                    <rdf:Description rdf:about="https://w3id.org/digitalconstruction/0.5/Entities#IndependentContinuant"/>
                    <owl:Class>
                        <owl:complementOf rdf:resource="https://w3id.org/digitalconstruction/0.5/Entities#SpatialRegion"/>
                    </owl:Class>
                </owl:intersectionOf>
            </owl:Class>
        </rdfs:domain>
        <rdfs:range>
            <owl:Class>
                <owl:intersectionOf rdf:parseType="Collection">
                    <rdf:Description rdf:about="https://w3id.org/digitalconstruction/0.5/Entities#IndependentContinuant"/>
                    <owl:Class>
                        <owl:complementOf rdf:resource="https://w3id.org/digitalconstruction/0.5/Entities#SpatialRegion"/>
                    </owl:Class>
                </owl:intersectionOf>
            </owl:Class>
        </rdfs:range>
        <rdfs:comment>locatedIn is equivalent to the BFO property &apos;located in at some time&apos; (http://purl.obolibrary.org/obo/BFO_0000171)</rdfs:comment>
        <rdfs:label>locatedIn</rdfs:label>
    </owl:ObjectProperty>
    


    <!-- https://w3id.org/digitalconstruction/0.5/Entities#locatedInAtAllTimes -->

    <owl:ObjectProperty rdf:about="https://w3id.org/digitalconstruction/0.5/Entities#locatedInAtAllTimes">
        <rdfs:subPropertyOf rdf:resource="https://w3id.org/digitalconstruction/0.5/Entities#locatedIn"/>
        <rdf:type rdf:resource="http://www.w3.org/2002/07/owl#TransitiveProperty"/>
        <rdfs:domain>
            <owl:Class>
                <owl:intersectionOf rdf:parseType="Collection">
                    <rdf:Description rdf:about="https://w3id.org/digitalconstruction/0.5/Entities#IndependentContinuant"/>
                    <owl:Class>
                        <owl:complementOf rdf:resource="https://w3id.org/digitalconstruction/0.5/Entities#SpatialRegion"/>
                    </owl:Class>
                </owl:intersectionOf>
            </owl:Class>
        </rdfs:domain>
        <rdfs:range>
            <owl:Class>
                <owl:intersectionOf rdf:parseType="Collection">
                    <rdf:Description rdf:about="https://w3id.org/digitalconstruction/0.5/Entities#IndependentContinuant"/>
                    <owl:Class>
                        <owl:complementOf rdf:resource="https://w3id.org/digitalconstruction/0.5/Entities#SpatialRegion"/>
                    </owl:Class>
                </owl:intersectionOf>
            </owl:Class>
        </rdfs:range>
        <rdfs:comment>locatedInAtAllTimes is equivalent to the BFO property &apos;located in at all times&apos; (http://purl.obolibrary.org/obo/BFO_0000082)</rdfs:comment>
        <rdfs:label>locatedInAtAllTimes</rdfs:label>
    </owl:ObjectProperty>
    


    <!-- https://w3id.org/digitalconstruction/0.5/Entities#locationOf -->

    <owl:ObjectProperty rdf:about="https://w3id.org/digitalconstruction/0.5/Entities#locationOf">
        <rdfs:domain>
            <owl:Class>
                <owl:intersectionOf rdf:parseType="Collection">
                    <rdf:Description rdf:about="https://w3id.org/digitalconstruction/0.5/Entities#IndependentContinuant"/>
                    <owl:Class>
                        <owl:complementOf rdf:resource="https://w3id.org/digitalconstruction/0.5/Entities#SpatialRegion"/>
                    </owl:Class>
                </owl:intersectionOf>
            </owl:Class>
        </rdfs:domain>
        <rdfs:range>
            <owl:Class>
                <owl:intersectionOf rdf:parseType="Collection">
                    <rdf:Description rdf:about="https://w3id.org/digitalconstruction/0.5/Entities#IndependentContinuant"/>
                    <owl:Class>
                        <owl:complementOf rdf:resource="https://w3id.org/digitalconstruction/0.5/Entities#SpatialRegion"/>
                    </owl:Class>
                </owl:intersectionOf>
            </owl:Class>
        </rdfs:range>
        <rdfs:comment>locationOf is equivalent to the BFO property &apos;location of at some time&apos; (http://purl.obolibrary.org/obo/BFO_0000124)</rdfs:comment>
        <rdfs:label>locationOf</rdfs:label>
    </owl:ObjectProperty>
    


    <!-- https://w3id.org/digitalconstruction/0.5/Entities#locationOfAtAllTimes -->

    <owl:ObjectProperty rdf:about="https://w3id.org/digitalconstruction/0.5/Entities#locationOfAtAllTimes">
        <rdfs:subPropertyOf rdf:resource="https://w3id.org/digitalconstruction/0.5/Entities#locationOf"/>
        <rdf:type rdf:resource="http://www.w3.org/2002/07/owl#TransitiveProperty"/>
        <rdfs:domain>
            <owl:Class>
                <owl:intersectionOf rdf:parseType="Collection">
                    <rdf:Description rdf:about="https://w3id.org/digitalconstruction/0.5/Entities#IndependentContinuant"/>
                    <owl:Class>
                        <owl:complementOf rdf:resource="https://w3id.org/digitalconstruction/0.5/Entities#SpatialRegion"/>
                    </owl:Class>
                </owl:intersectionOf>
            </owl:Class>
        </rdfs:domain>
        <rdfs:range>
            <owl:Class>
                <owl:intersectionOf rdf:parseType="Collection">
                    <rdf:Description rdf:about="https://w3id.org/digitalconstruction/0.5/Entities#IndependentContinuant"/>
                    <owl:Class>
                        <owl:complementOf rdf:resource="https://w3id.org/digitalconstruction/0.5/Entities#SpatialRegion"/>
                    </owl:Class>
                </owl:intersectionOf>
            </owl:Class>
        </rdfs:range>
        <rdfs:comment>locationOfAtAllTimes is equivalent to the BFO property &apos;location of at all times&apos; (http://purl.obolibrary.org/obo/BFO_0000170)</rdfs:comment>
        <rdfs:label>locationOfAtAllTimes</rdfs:label>
    </owl:ObjectProperty>
    


    <!-- https://w3id.org/digitalconstruction/0.5/Entities#materialBasisOf -->

    <owl:ObjectProperty rdf:about="https://w3id.org/digitalconstruction/0.5/Entities#materialBasisOf">
        <rdfs:domain rdf:resource="https://w3id.org/digitalconstruction/0.5/Entities#MaterialEntity"/>
        <rdfs:range rdf:resource="https://w3id.org/digitalconstruction/0.5/Entities#Disposition"/>
        <rdfs:comment>materialBasisOf is equivalent to the BFO property &apos;material basis of at some time&apos; (http://purl.obolibrary.org/obo/BFO_0000127)</rdfs:comment>
        <rdfs:label>materialBasisOf</rdfs:label>
    </owl:ObjectProperty>
    


    <!-- https://w3id.org/digitalconstruction/0.5/Entities#materialBasisOfAtAllTimes -->

    <owl:ObjectProperty rdf:about="https://w3id.org/digitalconstruction/0.5/Entities#materialBasisOfAtAllTimes">
        <rdfs:subPropertyOf rdf:resource="https://w3id.org/digitalconstruction/0.5/Entities#materialBasisOf"/>
        <rdfs:domain rdf:resource="https://w3id.org/digitalconstruction/0.5/Entities#MaterialEntity"/>
        <rdfs:range rdf:resource="https://w3id.org/digitalconstruction/0.5/Entities#Disposition"/>
        <rdfs:comment>materialBasisOfAtAllTimes is equivalent to the BFO property &apos;material basis of at all times&apos; (http://purl.obolibrary.org/obo/BFO_0000163)</rdfs:comment>
        <rdfs:label>materialBasisOfAtAllTimes</rdfs:label>
    </owl:ObjectProperty>
    


    <!-- https://w3id.org/digitalconstruction/0.5/Entities#memberOf -->

    <owl:ObjectProperty rdf:about="https://w3id.org/digitalconstruction/0.5/Entities#memberOf">
        <rdfs:domain rdf:resource="https://w3id.org/digitalconstruction/0.5/Entities#Entity"/>
        <rdfs:range rdf:resource="https://w3id.org/digitalconstruction/0.5/Entities#Group"/>
        <rdfs:label>memberOf</rdfs:label>
    </owl:ObjectProperty>
    


    <!-- https://w3id.org/digitalconstruction/0.5/Entities#memberPartOf -->

    <owl:ObjectProperty rdf:about="https://w3id.org/digitalconstruction/0.5/Entities#memberPartOf">
        <rdfs:subPropertyOf rdf:resource="https://w3id.org/digitalconstruction/0.5/Entities#continuantPartOf"/>
        <rdfs:domain rdf:resource="https://w3id.org/digitalconstruction/0.5/Entities#MaterialEntity"/>
        <rdfs:range rdf:resource="https://w3id.org/digitalconstruction/0.5/Entities#MaterialEntity"/>
        <rdfs:comment>memberPartOf is equivalent to the BFO property &apos;member part of at some time&apos; (http://purl.obolibrary.org/obo/BFO_0000129)</rdfs:comment>
        <rdfs:label>memberPartOf</rdfs:label>
    </owl:ObjectProperty>
    


    <!-- https://w3id.org/digitalconstruction/0.5/Entities#memberPartOfAtAllTimes -->

    <owl:ObjectProperty rdf:about="https://w3id.org/digitalconstruction/0.5/Entities#memberPartOfAtAllTimes">
        <rdfs:subPropertyOf rdf:resource="https://w3id.org/digitalconstruction/0.5/Entities#continuantPartOfAtAllTimes"/>
        <rdfs:subPropertyOf rdf:resource="https://w3id.org/digitalconstruction/0.5/Entities#memberPartOf"/>
        <rdfs:domain rdf:resource="https://w3id.org/digitalconstruction/0.5/Entities#MaterialEntity"/>
        <rdfs:range rdf:resource="https://w3id.org/digitalconstruction/0.5/Entities#MaterialEntity"/>
        <rdfs:comment>memberPartOfAtAllTimes is equivalent to the BFO property &apos;member part of at all times&apos; (http://purl.obolibrary.org/obo/BFO_0000173)</rdfs:comment>
        <rdfs:label>memberPartOfAtAllTimes</rdfs:label>
    </owl:ObjectProperty>
    


    <!-- https://w3id.org/digitalconstruction/0.5/Entities#occupiesSpatialRegion -->

    <owl:ObjectProperty rdf:about="https://w3id.org/digitalconstruction/0.5/Entities#occupiesSpatialRegion">
        <rdfs:domain>
            <owl:Class>
                <owl:intersectionOf rdf:parseType="Collection">
                    <rdf:Description rdf:about="https://w3id.org/digitalconstruction/0.5/Entities#IndependentContinuant"/>
                    <owl:Class>
                        <owl:complementOf rdf:resource="https://w3id.org/digitalconstruction/0.5/Entities#SpatialRegion"/>
                    </owl:Class>
                </owl:intersectionOf>
            </owl:Class>
        </rdfs:domain>
        <rdfs:range rdf:resource="https://w3id.org/digitalconstruction/0.5/Entities#SpatialRegion"/>
        <rdfs:comment>occupiesSpatialRegion is equivalent to the BFO property &apos;occupies spatial region at some time&apos; (http://purl.obolibrary.org/obo/BFO_0000210)</rdfs:comment>
        <rdfs:label>occupiesSpatialRegion</rdfs:label>
    </owl:ObjectProperty>
    


    <!-- https://w3id.org/digitalconstruction/0.5/Entities#occupiesSpatialRegionAtAllTimes -->

    <owl:ObjectProperty rdf:about="https://w3id.org/digitalconstruction/0.5/Entities#occupiesSpatialRegionAtAllTimes">
        <rdfs:subPropertyOf rdf:resource="https://w3id.org/digitalconstruction/0.5/Entities#occupiesSpatialRegion"/>
        <rdf:type rdf:resource="http://www.w3.org/2002/07/owl#FunctionalProperty"/>
        <rdfs:domain>
            <owl:Class>
                <owl:intersectionOf rdf:parseType="Collection">
                    <rdf:Description rdf:about="https://w3id.org/digitalconstruction/0.5/Entities#IndependentContinuant"/>
                    <owl:Class>
                        <owl:complementOf rdf:resource="https://w3id.org/digitalconstruction/0.5/Entities#SpatialRegion"/>
                    </owl:Class>
                </owl:intersectionOf>
            </owl:Class>
        </rdfs:domain>
        <rdfs:range rdf:resource="https://w3id.org/digitalconstruction/0.5/Entities#SpatialRegion"/>
        <rdfs:comment>occupiesSpatialRegionAtAllTimes is equivalent to the BFO property &apos;occupies spatial region at all times&apos; (http://purl.obolibrary.org/obo/BFO_0000211)</rdfs:comment>
        <rdfs:label>occupiesSpatialRegionAtAllTimes</rdfs:label>
    </owl:ObjectProperty>
    


    <!-- https://w3id.org/digitalconstruction/0.5/Entities#occupiesSpatiotemporalRegion -->

    <owl:ObjectProperty rdf:about="https://w3id.org/digitalconstruction/0.5/Entities#occupiesSpatiotemporalRegion">
        <rdf:type rdf:resource="http://www.w3.org/2002/07/owl#FunctionalProperty"/>
        <rdfs:domain>
            <owl:Class>
                <owl:unionOf rdf:parseType="Collection">
                    <rdf:Description rdf:about="https://w3id.org/digitalconstruction/0.5/Entities#Process"/>
                    <rdf:Description rdf:about="https://w3id.org/digitalconstruction/0.5/Entities#ProcessBoundary"/>
                </owl:unionOf>
            </owl:Class>
        </rdfs:domain>
        <rdfs:range rdf:resource="https://w3id.org/digitalconstruction/0.5/Entities#SpatiotemporalRegion"/>
        <rdfs:comment>occupiesSpatiotemporalRegion is equivalent to the BFO property &apos;occupies spatiotemporal region&apos; (http://purl.obolibrary.org/obo/BFO_0000200)</rdfs:comment>
        <rdfs:label>occupiesSpatiotemporalRegion</rdfs:label>
    </owl:ObjectProperty>
    


    <!-- https://w3id.org/digitalconstruction/0.5/Entities#occupiesTemporalRegion -->

    <owl:ObjectProperty rdf:about="https://w3id.org/digitalconstruction/0.5/Entities#occupiesTemporalRegion">
        <rdf:type rdf:resource="http://www.w3.org/2002/07/owl#FunctionalProperty"/>
        <rdfs:domain>
            <owl:Class>
                <owl:unionOf rdf:parseType="Collection">
                    <rdf:Description rdf:about="https://w3id.org/digitalconstruction/0.5/Entities#Process"/>
                    <rdf:Description rdf:about="https://w3id.org/digitalconstruction/0.5/Entities#ProcessBoundary"/>
                </owl:unionOf>
            </owl:Class>
        </rdfs:domain>
        <rdfs:range rdf:resource="https://w3id.org/digitalconstruction/0.5/Entities#TemporalRegion"/>
        <rdfs:comment>occupiesTemporalRegion is equivalent to the BFO property &apos;occupies temporal region&apos; (http://purl.obolibrary.org/obo/BFO_0000199)</rdfs:comment>
        <rdfs:label>occupiesTemporalRegion</rdfs:label>
    </owl:ObjectProperty>
    


    <!-- https://w3id.org/digitalconstruction/0.5/Entities#occurrentPartOf -->

    <owl:ObjectProperty rdf:about="https://w3id.org/digitalconstruction/0.5/Entities#occurrentPartOf">
        <rdfs:subPropertyOf rdf:resource="https://w3id.org/digitalconstruction/0.5/Entities#isPartOf"/>
        <rdf:type rdf:resource="http://www.w3.org/2002/07/owl#TransitiveProperty"/>
        <rdfs:domain rdf:resource="https://w3id.org/digitalconstruction/0.5/Entities#Occurrent"/>
        <rdfs:range rdf:resource="https://w3id.org/digitalconstruction/0.5/Entities#Occurrent"/>
        <rdfs:comment>occurrentPartOf is equivalent to the BFO property &apos;occurrent part of&apos; (http://purl.obolibrary.org/obo/BFO_0000132)</rdfs:comment>
        <rdfs:label>occurrentPartOf</rdfs:label>
    </owl:ObjectProperty>
    


    <!-- https://w3id.org/digitalconstruction/0.5/Entities#occursIn -->

    <owl:ObjectProperty rdf:about="https://w3id.org/digitalconstruction/0.5/Entities#occursIn">
        <rdfs:domain>
            <owl:Class>
                <owl:unionOf rdf:parseType="Collection">
                    <rdf:Description rdf:about="https://w3id.org/digitalconstruction/0.5/Entities#Process"/>
                    <rdf:Description rdf:about="https://w3id.org/digitalconstruction/0.5/Entities#ProcessBoundary"/>
                </owl:unionOf>
            </owl:Class>
        </rdfs:domain>
        <rdfs:range>
            <owl:Class>
                <owl:unionOf rdf:parseType="Collection">
                    <rdf:Description rdf:about="https://w3id.org/digitalconstruction/0.5/Entities#MaterialEntity"/>
                    <rdf:Description rdf:about="https://w3id.org/digitalconstruction/0.5/Entities#Site"/>
                </owl:unionOf>
            </owl:Class>
        </rdfs:range>
        <rdfs:comment>occursIn is equivalent to the BFO property &apos;occurs in&apos; (http://purl.obolibrary.org/obo/BFO_0000066)</rdfs:comment>
        <rdfs:label>occursIn</rdfs:label>
    </owl:ObjectProperty>
    


    <!-- https://w3id.org/digitalconstruction/0.5/Entities#participatesIn -->

    <owl:ObjectProperty rdf:about="https://w3id.org/digitalconstruction/0.5/Entities#participatesIn">
        <rdfs:domain>
            <owl:Class>
                <owl:unionOf rdf:parseType="Collection">
                    <rdf:Description rdf:about="https://w3id.org/digitalconstruction/0.5/Entities#GenericallyDependentContinuant"/>
                    <rdf:Description rdf:about="https://w3id.org/digitalconstruction/0.5/Entities#SpecificallyDependentContinuant"/>
                    <owl:Class>
                        <owl:intersectionOf rdf:parseType="Collection">
                            <rdf:Description rdf:about="https://w3id.org/digitalconstruction/0.5/Entities#IndependentContinuant"/>
                            <owl:Class>
                                <owl:complementOf rdf:resource="https://w3id.org/digitalconstruction/0.5/Entities#SpatialRegion"/>
                            </owl:Class>
                        </owl:intersectionOf>
                    </owl:Class>
                </owl:unionOf>
            </owl:Class>
        </rdfs:domain>
        <rdfs:range rdf:resource="https://w3id.org/digitalconstruction/0.5/Entities#Process"/>
        <rdfs:comment>participatesIn is equivalent to the BFO property &apos;participates in at some time&apos; (http://purl.obolibrary.org/obo/BFO_0000056)</rdfs:comment>
        <rdfs:label>participatesIn</rdfs:label>
    </owl:ObjectProperty>
    


    <!-- https://w3id.org/digitalconstruction/0.5/Entities#participatesInAtAllTimes -->

    <owl:ObjectProperty rdf:about="https://w3id.org/digitalconstruction/0.5/Entities#participatesInAtAllTimes">
        <rdfs:subPropertyOf rdf:resource="https://w3id.org/digitalconstruction/0.5/Entities#participatesIn"/>
        <rdfs:domain>
            <owl:Class>
                <owl:unionOf rdf:parseType="Collection">
                    <rdf:Description rdf:about="https://w3id.org/digitalconstruction/0.5/Entities#GenericallyDependentContinuant"/>
                    <rdf:Description rdf:about="https://w3id.org/digitalconstruction/0.5/Entities#SpecificallyDependentContinuant"/>
                    <owl:Class>
                        <owl:intersectionOf rdf:parseType="Collection">
                            <rdf:Description rdf:about="https://w3id.org/digitalconstruction/0.5/Entities#IndependentContinuant"/>
                            <owl:Class>
                                <owl:complementOf rdf:resource="https://w3id.org/digitalconstruction/0.5/Entities#SpatialRegion"/>
                            </owl:Class>
                        </owl:intersectionOf>
                    </owl:Class>
                </owl:unionOf>
            </owl:Class>
        </rdfs:domain>
        <rdfs:range rdf:resource="https://w3id.org/digitalconstruction/0.5/Entities#Process"/>
        <rdfs:comment>participatesInAtAllTimes is equivalent to the BFO property &apos;participates in at all times&apos; (http://purl.obolibrary.org/obo/BFO_0000166)</rdfs:comment>
        <rdfs:label>participatesInAtAllTimes</rdfs:label>
    </owl:ObjectProperty>
    


    <!-- https://w3id.org/digitalconstruction/0.5/Entities#precededBy -->

    <owl:ObjectProperty rdf:about="https://w3id.org/digitalconstruction/0.5/Entities#precededBy">
        <rdf:type rdf:resource="http://www.w3.org/2002/07/owl#TransitiveProperty"/>
        <rdfs:domain rdf:resource="https://w3id.org/digitalconstruction/0.5/Entities#Occurrent"/>
        <rdfs:range rdf:resource="https://w3id.org/digitalconstruction/0.5/Entities#Occurrent"/>
        <rdfs:comment>precededBy is equivalent to the BFO property &apos;preceded by&apos; (http://purl.obolibrary.org/obo/BFO_0000062)</rdfs:comment>
        <rdfs:label>precededBy</rdfs:label>
    </owl:ObjectProperty>
    


    <!-- https://w3id.org/digitalconstruction/0.5/Entities#precedes -->

    <owl:ObjectProperty rdf:about="https://w3id.org/digitalconstruction/0.5/Entities#precedes">
        <rdf:type rdf:resource="http://www.w3.org/2002/07/owl#TransitiveProperty"/>
        <rdfs:domain rdf:resource="https://w3id.org/digitalconstruction/0.5/Entities#Occurrent"/>
        <rdfs:range rdf:resource="https://w3id.org/digitalconstruction/0.5/Entities#Occurrent"/>
        <rdfs:comment>precedes is equivalent to the BFO property &apos;precedes&apos; (http://purl.obolibrary.org/obo/BFO_0000063)</rdfs:comment>
        <rdfs:label>precedes</rdfs:label>
    </owl:ObjectProperty>
    


    <!-- https://w3id.org/digitalconstruction/0.5/Entities#properContinuantPartOf -->

    <owl:ObjectProperty rdf:about="https://w3id.org/digitalconstruction/0.5/Entities#properContinuantPartOf">
        <rdfs:subPropertyOf rdf:resource="https://w3id.org/digitalconstruction/0.5/Entities#continuantPartOf"/>
        <rdfs:domain rdf:resource="https://w3id.org/digitalconstruction/0.5/Entities#Continuant"/>
        <rdfs:range rdf:resource="https://w3id.org/digitalconstruction/0.5/Entities#Continuant"/>
        <rdfs:comment>properContinuantPartOf is equivalent to the BFO property &apos;proper continuant part of at some time&apos; (http://purl.obolibrary.org/obo/BFO_0000175)</rdfs:comment>
        <rdfs:label>properContinuantPartOf</rdfs:label>
    </owl:ObjectProperty>
    


    <!-- https://w3id.org/digitalconstruction/0.5/Entities#properContinuantPartOfAtAllTimes -->

    <owl:ObjectProperty rdf:about="https://w3id.org/digitalconstruction/0.5/Entities#properContinuantPartOfAtAllTimes">
        <rdfs:subPropertyOf rdf:resource="https://w3id.org/digitalconstruction/0.5/Entities#continuantPartOfAtAllTimes"/>
        <rdfs:subPropertyOf rdf:resource="https://w3id.org/digitalconstruction/0.5/Entities#properContinuantPartOf"/>
        <rdf:type rdf:resource="http://www.w3.org/2002/07/owl#TransitiveProperty"/>
        <rdfs:domain rdf:resource="https://w3id.org/digitalconstruction/0.5/Entities#Continuant"/>
        <rdfs:range rdf:resource="https://w3id.org/digitalconstruction/0.5/Entities#Continuant"/>
        <rdfs:comment>properContinuantPartOfAtAllTimes is equivalent to the BFO property &apos;proper continuant part of at all times&apos; (http://purl.obolibrary.org/obo/BFO_0000137)</rdfs:comment>
        <rdfs:label>properContinuantPartOfAtAllTimes</rdfs:label>
    </owl:ObjectProperty>
    


    <!-- https://w3id.org/digitalconstruction/0.5/Entities#properOccurrentPartOf -->

    <owl:ObjectProperty rdf:about="https://w3id.org/digitalconstruction/0.5/Entities#properOccurrentPartOf">
        <rdfs:subPropertyOf rdf:resource="https://w3id.org/digitalconstruction/0.5/Entities#occurrentPartOf"/>
        <rdfs:domain rdf:resource="https://w3id.org/digitalconstruction/0.5/Entities#Occurrent"/>
        <rdfs:range rdf:resource="https://w3id.org/digitalconstruction/0.5/Entities#Occurrent"/>
        <rdfs:comment>properOccurrentPartOf is equivalent to the BFO property &apos;proper occurrent part of&apos; (http://purl.obolibrary.org/obo/BFO_0000138)</rdfs:comment>
        <rdfs:label>properOccurrentPartOf</rdfs:label>
    </owl:ObjectProperty>
    


    <!-- https://w3id.org/digitalconstruction/0.5/Entities#properTemporalPartOf -->

    <owl:ObjectProperty rdf:about="https://w3id.org/digitalconstruction/0.5/Entities#properTemporalPartOf">
        <rdfs:subPropertyOf rdf:resource="https://w3id.org/digitalconstruction/0.5/Entities#temporalPartOf"/>
        <rdfs:domain rdf:resource="https://w3id.org/digitalconstruction/0.5/Entities#Occurrent"/>
        <rdfs:range rdf:resource="https://w3id.org/digitalconstruction/0.5/Entities#Occurrent"/>
        <rdfs:comment>properTemporalPartOf is equivalent to the BFO property &apos;proper temporal part of&apos; (http://purl.obolibrary.org/obo/BFO_0000136)</rdfs:comment>
        <rdfs:label>properTemporalPartOf</rdfs:label>
    </owl:ObjectProperty>
    


    <!-- https://w3id.org/digitalconstruction/0.5/Entities#realizes -->

    <owl:ObjectProperty rdf:about="https://w3id.org/digitalconstruction/0.5/Entities#realizes">
        <rdfs:domain rdf:resource="https://w3id.org/digitalconstruction/0.5/Entities#Process"/>
        <rdfs:range rdf:resource="https://w3id.org/digitalconstruction/0.5/Entities#RealizableEntity"/>
        <rdfs:comment>realizes is equivalent to the BFO property &apos;realizes&apos; (http://purl.obolibrary.org/obo/BFO_0000055)</rdfs:comment>
        <rdfs:label>realizes</rdfs:label>
    </owl:ObjectProperty>
    


    <!-- https://w3id.org/digitalconstruction/0.5/Entities#spatiallyProjectsOnto -->

    <owl:ObjectProperty rdf:about="https://w3id.org/digitalconstruction/0.5/Entities#spatiallyProjectsOnto">
        <rdfs:domain rdf:resource="https://w3id.org/digitalconstruction/0.5/Entities#SpatiotemporalRegion"/>
        <rdfs:range rdf:resource="https://w3id.org/digitalconstruction/0.5/Entities#SpatialRegion"/>
        <rdfs:comment>spatiallyProjectsOnto is equivalent to the BFO property &apos;spatially projects onto at some time&apos; (http://purl.obolibrary.org/obo/BFO_0000216)</rdfs:comment>
        <rdfs:label>spatiallyProjectsOnto</rdfs:label>
    </owl:ObjectProperty>
    


    <!-- https://w3id.org/digitalconstruction/0.5/Entities#spatiallyProjectsOntoAtAllTimes -->

    <owl:ObjectProperty rdf:about="https://w3id.org/digitalconstruction/0.5/Entities#spatiallyProjectsOntoAtAllTimes">
        <rdfs:subPropertyOf rdf:resource="https://w3id.org/digitalconstruction/0.5/Entities#spatiallyProjectsOnto"/>
        <rdf:type rdf:resource="http://www.w3.org/2002/07/owl#FunctionalProperty"/>
        <rdfs:domain rdf:resource="https://w3id.org/digitalconstruction/0.5/Entities#SpatiotemporalRegion"/>
        <rdfs:range rdf:resource="https://w3id.org/digitalconstruction/0.5/Entities#SpatialRegion"/>
        <rdfs:comment>spatiallyProjectsOntoAtAllTimes is equivalent to the BFO property &apos;spatially projects onto at all times&apos; (http://purl.obolibrary.org/obo/BFO_0000217)</rdfs:comment>
        <rdfs:label>spatiallyProjectsOntoAtAllTimes</rdfs:label>
    </owl:ObjectProperty>
    


    <!-- https://w3id.org/digitalconstruction/0.5/Entities#specificallyDependedOnBy -->

    <owl:ObjectProperty rdf:about="https://w3id.org/digitalconstruction/0.5/Entities#specificallyDependedOnBy">
        <rdfs:domain>
            <owl:Class>
                <owl:unionOf rdf:parseType="Collection">
                    <rdf:Description rdf:about="https://w3id.org/digitalconstruction/0.5/Entities#SpecificallyDependentContinuant"/>
                    <owl:Class>
                        <owl:intersectionOf rdf:parseType="Collection">
                            <rdf:Description rdf:about="https://w3id.org/digitalconstruction/0.5/Entities#IndependentContinuant"/>
                            <owl:Class>
                                <owl:complementOf rdf:resource="https://w3id.org/digitalconstruction/0.5/Entities#SpatialRegion"/>
                            </owl:Class>
                        </owl:intersectionOf>
                    </owl:Class>
                </owl:unionOf>
            </owl:Class>
        </rdfs:domain>
        <rdfs:range rdf:resource="https://w3id.org/digitalconstruction/0.5/Entities#SpecificallyDependentContinuant"/>
        <rdfs:comment>specificallyDependedOnBy is equivalent to the BFO property &apos;specifically depended on by&apos; (http://purl.obolibrary.org/obo/BFO_0000194)</rdfs:comment>
        <rdfs:label>specificallyDependedOnBy</rdfs:label>
    </owl:ObjectProperty>
    


    <!-- https://w3id.org/digitalconstruction/0.5/Entities#specificallyDependsOn -->

    <owl:ObjectProperty rdf:about="https://w3id.org/digitalconstruction/0.5/Entities#specificallyDependsOn">
        <rdfs:domain rdf:resource="https://w3id.org/digitalconstruction/0.5/Entities#SpecificallyDependentContinuant"/>
        <rdfs:range>
            <owl:Class>
                <owl:unionOf rdf:parseType="Collection">
                    <rdf:Description rdf:about="https://w3id.org/digitalconstruction/0.5/Entities#SpecificallyDependentContinuant"/>
                    <owl:Class>
                        <owl:intersectionOf rdf:parseType="Collection">
                            <rdf:Description rdf:about="https://w3id.org/digitalconstruction/0.5/Entities#IndependentContinuant"/>
                            <owl:Class>
                                <owl:complementOf rdf:resource="https://w3id.org/digitalconstruction/0.5/Entities#SpatialRegion"/>
                            </owl:Class>
                        </owl:intersectionOf>
                    </owl:Class>
                </owl:unionOf>
            </owl:Class>
        </rdfs:range>
        <rdfs:comment>specificallyDependsOn is equivalent to the BFO property &apos;specifically depends on&apos; (http://purl.obolibrary.org/obo/BFO_0000195)</rdfs:comment>
        <rdfs:label>specificallyDependsOn</rdfs:label>
    </owl:ObjectProperty>
    


    <!-- https://w3id.org/digitalconstruction/0.5/Entities#temporalPartOf -->

    <owl:ObjectProperty rdf:about="https://w3id.org/digitalconstruction/0.5/Entities#temporalPartOf">
        <rdfs:subPropertyOf rdf:resource="https://w3id.org/digitalconstruction/0.5/Entities#occurrentPartOf"/>
        <rdf:type rdf:resource="http://www.w3.org/2002/07/owl#TransitiveProperty"/>
        <rdfs:domain rdf:resource="https://w3id.org/digitalconstruction/0.5/Entities#Occurrent"/>
        <rdfs:range rdf:resource="https://w3id.org/digitalconstruction/0.5/Entities#Occurrent"/>
        <rdfs:comment>temporalPartOf is equivalent to the BFO property &apos;temporal part of&apos; (http://purl.obolibrary.org/obo/BFO_0000139)</rdfs:comment>
        <rdfs:label>temporalPartOf</rdfs:label>
    </owl:ObjectProperty>
    


    <!-- https://w3id.org/digitalconstruction/0.5/Entities#temporallyProjectsOnto -->

    <owl:ObjectProperty rdf:about="https://w3id.org/digitalconstruction/0.5/Entities#temporallyProjectsOnto">
        <rdf:type rdf:resource="http://www.w3.org/2002/07/owl#FunctionalProperty"/>
        <rdfs:domain rdf:resource="https://w3id.org/digitalconstruction/0.5/Entities#SpatiotemporalRegion"/>
        <rdfs:range rdf:resource="https://w3id.org/digitalconstruction/0.5/Entities#TemporalRegion"/>
        <rdfs:comment>temporallyProjectsOnto is equivalent to the BFO property &apos;temporally projects onto&apos; (http://purl.obolibrary.org/obo/BFO_0000153)</rdfs:comment>
        <rdfs:label>temporallyProjectsOnto</rdfs:label>
    </owl:ObjectProperty>
    


    <!-- https://w3id.org/digitalconstruction/0.5/Variables#hasProperty -->

    <owl:ObjectProperty rdf:about="https://w3id.org/digitalconstruction/0.5/Variables#hasProperty"/>
    


    <!-- https://w3id.org/digitalconstruction/0.5/Variables#isPropertyOf -->

    <owl:ObjectProperty rdf:about="https://w3id.org/digitalconstruction/0.5/Variables#isPropertyOf"/>
    


    <!-- 
    ///////////////////////////////////////////////////////////////////////////////////////
    //
    // Data properties
    //
    ///////////////////////////////////////////////////////////////////////////////////////
     -->

    


    <!-- https://w3id.org/digitalconstruction/0.5/Entities#hasAltitude -->

    <owl:DatatypeProperty rdf:about="https://w3id.org/digitalconstruction/0.5/Entities#hasAltitude">
        <rdfs:domain>
            <owl:Class>
                <owl:unionOf rdf:parseType="Collection">
                    <rdf:Description rdf:about="https://w3id.org/digitalconstruction/0.5/Entities#GeodeticPosition"/>
                    <rdf:Description rdf:about="https://w3id.org/digitalconstruction/0.5/Entities#SpatialRegion"/>
                </owl:unionOf>
            </owl:Class>
        </rdfs:domain>
        <rdfs:range rdf:resource="http://www.w3.org/2001/XMLSchema#decimal"/>
        <rdfs:label>hasAltitude</rdfs:label>
    </owl:DatatypeProperty>
    


    <!-- https://w3id.org/digitalconstruction/0.5/Entities#hasDipAngle -->

    <owl:DatatypeProperty rdf:about="https://w3id.org/digitalconstruction/0.5/Entities#hasDipAngle">
        <rdfs:domain rdf:resource="https://w3id.org/digitalconstruction/0.5/Entities#TwoAngleOrientation"/>
        <rdfs:range rdf:resource="http://www.w3.org/2001/XMLSchema#double"/>
        <rdfs:label>hasDipAngle</rdfs:label>
    </owl:DatatypeProperty>
    


    <!-- https://w3id.org/digitalconstruction/0.5/Entities#hasGeodeticCoordinateSystem -->

    <owl:DatatypeProperty rdf:about="https://w3id.org/digitalconstruction/0.5/Entities#hasGeodeticCoordinateSystem">
        <rdfs:domain rdf:resource="https://w3id.org/digitalconstruction/0.5/Entities#GeodeticPosition"/>
        <rdfs:range rdf:resource="http://www.w3.org/2001/XMLSchema#string"/>
        <rdfs:label>hasGeodeticCoordinateSystem</rdfs:label>
    </owl:DatatypeProperty>
    


    <!-- https://w3id.org/digitalconstruction/0.5/Entities#hasLabel -->

    <owl:DatatypeProperty rdf:about="https://w3id.org/digitalconstruction/0.5/Entities#hasLabel">
        <rdfs:domain rdf:resource="https://w3id.org/digitalconstruction/0.5/Entities#Labeling"/>
        <rdfs:range rdf:resource="http://www.w3.org/2001/XMLSchema#string"/>
        <rdfs:label>hasLabel</rdfs:label>
    </owl:DatatypeProperty>
    


    <!-- https://w3id.org/digitalconstruction/0.5/Entities#hasLatitude -->

    <owl:DatatypeProperty rdf:about="https://w3id.org/digitalconstruction/0.5/Entities#hasLatitude">
        <rdfs:domain>
            <owl:Class>
                <owl:unionOf rdf:parseType="Collection">
                    <rdf:Description rdf:about="https://w3id.org/digitalconstruction/0.5/Entities#GeodeticPosition"/>
                    <rdf:Description rdf:about="https://w3id.org/digitalconstruction/0.5/Entities#SpatialRegion"/>
                </owl:unionOf>
            </owl:Class>
        </rdfs:domain>
        <rdfs:range rdf:resource="http://www.w3.org/2001/XMLSchema#decimal"/>
        <rdfs:label>hasLatitude</rdfs:label>
    </owl:DatatypeProperty>
    


    <!-- https://w3id.org/digitalconstruction/0.5/Entities#hasLongitude -->

    <owl:DatatypeProperty rdf:about="https://w3id.org/digitalconstruction/0.5/Entities#hasLongitude">
        <rdfs:domain>
            <owl:Class>
                <owl:unionOf rdf:parseType="Collection">
                    <rdf:Description rdf:about="https://w3id.org/digitalconstruction/0.5/Entities#GeodeticPosition"/>
                    <rdf:Description rdf:about="https://w3id.org/digitalconstruction/0.5/Entities#SpatialRegion"/>
                </owl:unionOf>
            </owl:Class>
        </rdfs:domain>
        <rdfs:range rdf:resource="http://www.w3.org/2001/XMLSchema#decimal"/>
        <rdfs:label>hasLongitude</rdfs:label>
    </owl:DatatypeProperty>
    


    <!-- https://w3id.org/digitalconstruction/0.5/Entities#hasMaxLoad -->

    <owl:DatatypeProperty rdf:about="https://w3id.org/digitalconstruction/0.5/Entities#hasMaxLoad">
        <rdfs:domain rdf:resource="https://w3id.org/digitalconstruction/0.5/Entities#Vehicle"/>
        <rdfs:range rdf:resource="http://www.w3.org/2002/07/owl#real"/>
        <rdfs:label>hasMaxLoad</rdfs:label>
    </owl:DatatypeProperty>
    


    <!-- https://w3id.org/digitalconstruction/0.5/Entities#hasNorthAngle -->

    <owl:DatatypeProperty rdf:about="https://w3id.org/digitalconstruction/0.5/Entities#hasNorthAngle">
        <rdfs:domain rdf:resource="https://w3id.org/digitalconstruction/0.5/Entities#OneAngleOrientation"/>
        <rdfs:range rdf:resource="http://www.w3.org/2001/XMLSchema#double"/>
        <rdfs:label>hasNorthAngle</rdfs:label>
    </owl:DatatypeProperty>
    


    <!-- https://w3id.org/digitalconstruction/0.5/Entities#hasStrikeAngle -->

    <owl:DatatypeProperty rdf:about="https://w3id.org/digitalconstruction/0.5/Entities#hasStrikeAngle">
        <rdfs:domain rdf:resource="https://w3id.org/digitalconstruction/0.5/Entities#TwoAngleOrientation"/>
        <rdfs:range rdf:resource="http://www.w3.org/2001/XMLSchema#double"/>
        <rdfs:label>hasStrikeAngle</rdfs:label>
    </owl:DatatypeProperty>
    


    <!-- https://w3id.org/digitalconstruction/0.5/Entities#hasX -->

    <owl:DatatypeProperty rdf:about="https://w3id.org/digitalconstruction/0.5/Entities#hasX">
        <rdfs:domain rdf:resource="https://w3id.org/digitalconstruction/0.5/Entities#CartesianPosition"/>
        <rdfs:range rdf:resource="http://www.w3.org/2001/XMLSchema#double"/>
        <rdfs:label>hasX</rdfs:label>
    </owl:DatatypeProperty>
    


    <!-- https://w3id.org/digitalconstruction/0.5/Entities#hasXAngle -->

    <owl:DatatypeProperty rdf:about="https://w3id.org/digitalconstruction/0.5/Entities#hasXAngle">
        <rdfs:domain rdf:resource="https://w3id.org/digitalconstruction/0.5/Entities#ThreeAngleOrientation"/>
        <rdfs:range rdf:resource="http://www.w3.org/2001/XMLSchema#double"/>
        <rdfs:label>hasXAngle</rdfs:label>
    </owl:DatatypeProperty>
    


    <!-- https://w3id.org/digitalconstruction/0.5/Entities#hasXLength -->

    <owl:DatatypeProperty rdf:about="https://w3id.org/digitalconstruction/0.5/Entities#hasXLength">
        <rdfs:domain rdf:resource="https://w3id.org/digitalconstruction/0.5/Entities#CartesianVolume"/>
        <rdfs:range rdf:resource="http://www.w3.org/2001/XMLSchema#double"/>
        <rdfs:label>hasXLength</rdfs:label>
    </owl:DatatypeProperty>
    


    <!-- https://w3id.org/digitalconstruction/0.5/Entities#hasY -->

    <owl:DatatypeProperty rdf:about="https://w3id.org/digitalconstruction/0.5/Entities#hasY">
        <rdfs:domain rdf:resource="https://w3id.org/digitalconstruction/0.5/Entities#CartesianPosition"/>
        <rdfs:range rdf:resource="http://www.w3.org/2001/XMLSchema#double"/>
        <rdfs:label>hasY</rdfs:label>
    </owl:DatatypeProperty>
    


    <!-- https://w3id.org/digitalconstruction/0.5/Entities#hasYAngle -->

    <owl:DatatypeProperty rdf:about="https://w3id.org/digitalconstruction/0.5/Entities#hasYAngle">
        <rdfs:domain rdf:resource="https://w3id.org/digitalconstruction/0.5/Entities#ThreeAngleOrientation"/>
        <rdfs:range rdf:resource="http://www.w3.org/2001/XMLSchema#double"/>
        <rdfs:label>hasYAngle</rdfs:label>
    </owl:DatatypeProperty>
    


    <!-- https://w3id.org/digitalconstruction/0.5/Entities#hasYLength -->

    <owl:DatatypeProperty rdf:about="https://w3id.org/digitalconstruction/0.5/Entities#hasYLength">
        <rdfs:domain rdf:resource="https://w3id.org/digitalconstruction/0.5/Entities#CartesianVolume"/>
        <rdfs:range rdf:resource="http://www.w3.org/2001/XMLSchema#double"/>
        <rdfs:label>hasYLength</rdfs:label>
    </owl:DatatypeProperty>
    


    <!-- https://w3id.org/digitalconstruction/0.5/Entities#hasZ -->

    <owl:DatatypeProperty rdf:about="https://w3id.org/digitalconstruction/0.5/Entities#hasZ">
        <rdfs:domain rdf:resource="https://w3id.org/digitalconstruction/0.5/Entities#CartesianPosition"/>
        <rdfs:range rdf:resource="http://www.w3.org/2001/XMLSchema#double"/>
        <rdfs:label>hasZ</rdfs:label>
    </owl:DatatypeProperty>
    


    <!-- https://w3id.org/digitalconstruction/0.5/Entities#hasZAngle -->

    <owl:DatatypeProperty rdf:about="https://w3id.org/digitalconstruction/0.5/Entities#hasZAngle">
        <rdfs:domain rdf:resource="https://w3id.org/digitalconstruction/0.5/Entities#ThreeAngleOrientation"/>
        <rdfs:range rdf:resource="http://www.w3.org/2001/XMLSchema#double"/>
        <rdfs:label>hasZAngle</rdfs:label>
    </owl:DatatypeProperty>
    


    <!-- https://w3id.org/digitalconstruction/0.5/Entities#hasZLength -->

    <owl:DatatypeProperty rdf:about="https://w3id.org/digitalconstruction/0.5/Entities#hasZLength">
        <rdfs:domain rdf:resource="https://w3id.org/digitalconstruction/0.5/Entities#CartesianVolume"/>
        <rdfs:range rdf:resource="http://www.w3.org/2001/XMLSchema#double"/>
        <rdfs:label>hasZLength</rdfs:label>
    </owl:DatatypeProperty>
    


    <!-- 
    ///////////////////////////////////////////////////////////////////////////////////////
    //
    // Classes
    //
    ///////////////////////////////////////////////////////////////////////////////////////
     -->

    


    <!-- https://w3id.org/digitalconstruction/0.5/Entities#Actuator -->

    <owl:Class rdf:about="https://w3id.org/digitalconstruction/0.5/Entities#Actuator">
        <rdfs:subClassOf rdf:resource="https://w3id.org/digitalconstruction/0.5/Entities#Device"/>
        <rdfs:label>Actuator</rdfs:label>
    </owl:Class>
    


    <!-- https://w3id.org/digitalconstruction/0.5/Entities#Asset -->

    <owl:Class rdf:about="https://w3id.org/digitalconstruction/0.5/Entities#Asset">
        <rdfs:subClassOf>
            <owl:Class>
                <owl:unionOf rdf:parseType="Collection">
                    <rdf:Description rdf:about="https://w3id.org/digitalconstruction/0.5/Entities#GenericallyDependentContinuant"/>
                    <rdf:Description rdf:about="https://w3id.org/digitalconstruction/0.5/Entities#MaterialEntity"/>
                    <rdf:Description rdf:about="https://w3id.org/digitalconstruction/0.5/Entities#Site"/>
                </owl:unionOf>
            </owl:Class>
        </rdfs:subClassOf>
        <rdfs:subClassOf>
            <owl:Restriction>
                <owl:onProperty rdf:resource="https://w3id.org/digitalconstruction/0.5/Entities#hasRole"/>
                <owl:someValuesFrom rdf:resource="https://w3id.org/digitalconstruction/0.5/Entities#AssetRole"/>
            </owl:Restriction>
        </rdfs:subClassOf>
        <rdfs:comment>Something that acts in the asset role</rdfs:comment>
        <rdfs:label>Asset</rdfs:label>
    </owl:Class>
    


    <!-- https://w3id.org/digitalconstruction/0.5/Entities#AssetRole -->

    <owl:Class rdf:about="https://w3id.org/digitalconstruction/0.5/Entities#AssetRole">
        <rdfs:subClassOf rdf:resource="https://w3id.org/digitalconstruction/0.5/Entities#Role"/>
        <rdfs:comment>A role in which an entity acts as an asset</rdfs:comment>
        <rdfs:label>AssetRole</rdfs:label>
    </owl:Class>
    


    <!-- https://w3id.org/digitalconstruction/0.5/Entities#Building -->

    <owl:Class rdf:about="https://w3id.org/digitalconstruction/0.5/Entities#Building">
        <rdfs:subClassOf rdf:resource="https://w3id.org/digitalconstruction/0.5/Entities#BuiltAsset"/>
        <rdfs:label>Building</rdfs:label>
    </owl:Class>
    


    <!-- https://w3id.org/digitalconstruction/0.5/Entities#BuildingObject -->

    <owl:Class rdf:about="https://w3id.org/digitalconstruction/0.5/Entities#BuildingObject">
        <rdfs:subClassOf rdf:resource="https://w3id.org/digitalconstruction/0.5/Entities#Object"/>
        <rdfs:comment>An entity that forms a part of an existing or designed building</rdfs:comment>
        <rdfs:label>BuildingObject</rdfs:label>
    </owl:Class>
    


    <!-- https://w3id.org/digitalconstruction/0.5/Entities#BuildingServiceSystem -->

    <owl:Class rdf:about="https://w3id.org/digitalconstruction/0.5/Entities#BuildingServiceSystem">
        <rdfs:subClassOf rdf:resource="https://w3id.org/digitalconstruction/0.5/Entities#ObjectAggregate"/>
        <rdfs:comment>A system of a building service. For example, a ventilation system or a heating system.</rdfs:comment>
        <rdfs:label>BuildingServiceSystem</rdfs:label>
    </owl:Class>
    


    <!-- https://w3id.org/digitalconstruction/0.5/Entities#BuildingUnit -->

    <owl:Class rdf:about="https://w3id.org/digitalconstruction/0.5/Entities#BuildingUnit">
        <rdfs:subClassOf rdf:resource="https://w3id.org/digitalconstruction/0.5/Entities#BuiltAsset"/>
        <rdfs:comment>A separately used part of a building</rdfs:comment>
    </owl:Class>
    


    <!-- https://w3id.org/digitalconstruction/0.5/Entities#BuiltAsset -->

    <owl:Class rdf:about="https://w3id.org/digitalconstruction/0.5/Entities#BuiltAsset">
        <rdfs:subClassOf rdf:resource="https://w3id.org/digitalconstruction/0.5/Entities#Asset"/>
        <rdfs:subClassOf rdf:resource="https://w3id.org/digitalconstruction/0.5/Entities#Location"/>
        <rdfs:comment>A location that is in a role of an asset. An asset that is part of the built environment (ISO 19650-1)</rdfs:comment>
        <rdfs:label>BuiltAsset</rdfs:label>
    </owl:Class>
    


    <!-- https://w3id.org/digitalconstruction/0.5/Entities#Capability -->

    <owl:Class rdf:about="https://w3id.org/digitalconstruction/0.5/Entities#Capability">
        <rdfs:subClassOf rdf:resource="https://w3id.org/digitalconstruction/0.5/Entities#Disposition"/>
        <rdfs:label>Capability</rdfs:label>
    </owl:Class>
    


    <!-- https://w3id.org/digitalconstruction/0.5/Entities#CartesianBoundingBox -->

    <owl:Class rdf:about="https://w3id.org/digitalconstruction/0.5/Entities#CartesianBoundingBox">
        <rdfs:subClassOf rdf:resource="https://w3id.org/digitalconstruction/0.5/Entities#SpatialExtent"/>
        <rdfs:comment>Minimum bounding box of an entity given by a minimum cartesian position and maximum cartesian position</rdfs:comment>
        <rdfs:label>CartesianBoundingBox</rdfs:label>
    </owl:Class>
    


    <!-- https://w3id.org/digitalconstruction/0.5/Entities#CartesianPosition -->

    <owl:Class rdf:about="https://w3id.org/digitalconstruction/0.5/Entities#CartesianPosition">
        <rdfs:subClassOf rdf:resource="https://w3id.org/digitalconstruction/0.5/Entities#SpatialPosition"/>
        <rdfs:comment>Cartesian position expressed as x, y, and z coordinates with respect to a spatial origin and spatial orientation</rdfs:comment>
        <rdfs:label>CartesianPosition</rdfs:label>
    </owl:Class>
    


    <!-- https://w3id.org/digitalconstruction/0.5/Entities#CartesianVolume -->

    <owl:Class rdf:about="https://w3id.org/digitalconstruction/0.5/Entities#CartesianVolume">
        <rdfs:subClassOf rdf:resource="https://w3id.org/digitalconstruction/0.5/Entities#SpatialExtent"/>
        <rdfs:comment>Cartesian volume given by the lengths to x, y, and z directions</rdfs:comment>
        <rdfs:label>CartesianVolume</rdfs:label>
    </owl:Class>
    


    <!-- https://w3id.org/digitalconstruction/0.5/Entities#Category -->

    <owl:Class rdf:about="https://w3id.org/digitalconstruction/0.5/Entities#Category">
        <rdfs:subClassOf rdf:resource="https://w3id.org/digitalconstruction/0.5/Entities#Labeling"/>
        <owl:disjointWith rdf:resource="https://w3id.org/digitalconstruction/0.5/Entities#Identifier"/>
        <rdfs:comment>Category is a labeling of an entity the associates it with some defined class of things. For example, an object can be associated with a particular class in a classification system such as OmniClass, UniFormat, CoClass, or Talo2000. Category allows also to associate an entity with a category of entities represented in an external system or belonging to a particular project.</rdfs:comment>
        <rdfs:label>Category</rdfs:label>
    </owl:Class>
    


    <!-- https://w3id.org/digitalconstruction/0.5/Entities#Continuant -->

    <owl:Class rdf:about="https://w3id.org/digitalconstruction/0.5/Entities#Continuant">
        <rdfs:subClassOf rdf:resource="https://w3id.org/digitalconstruction/0.5/Entities#Entity"/>
        <rdfs:subClassOf>
            <owl:Restriction>
                <owl:onProperty rdf:resource="https://w3id.org/digitalconstruction/0.5/Entities#continuantPartOfAtAllTimes"/>
                <owl:allValuesFrom rdf:resource="https://w3id.org/digitalconstruction/0.5/Entities#Continuant"/>
            </owl:Restriction>
        </rdfs:subClassOf>
        <owl:disjointWith rdf:resource="https://w3id.org/digitalconstruction/0.5/Entities#Occurrent"/>
        <rdfs:comment>Continuant is equivalent to the BFO class &apos;continuant&apos; (http://purl.obolibrary.org/obo/BFO_0000002)</rdfs:comment>
        <rdfs:label>Continuant</rdfs:label>
    </owl:Class>
    


    <!-- https://w3id.org/digitalconstruction/0.5/Entities#ContinuantFiatBoundary -->

    <owl:Class rdf:about="https://w3id.org/digitalconstruction/0.5/Entities#ContinuantFiatBoundary">
        <rdfs:subClassOf rdf:resource="https://w3id.org/digitalconstruction/0.5/Entities#ImmaterialEntity"/>
        <rdfs:subClassOf>
            <owl:Restriction>
                <owl:onProperty rdf:resource="https://w3id.org/digitalconstruction/0.5/Entities#hasContinuantPartAtAllTimes"/>
                <owl:allValuesFrom rdf:resource="https://w3id.org/digitalconstruction/0.5/Entities#ContinuantFiatBoundary"/>
            </owl:Restriction>
        </rdfs:subClassOf>
        <rdfs:subClassOf>
            <owl:Restriction>
                <owl:onProperty rdf:resource="https://w3id.org/digitalconstruction/0.5/Entities#locationOfAtAllTimes"/>
                <owl:allValuesFrom rdf:resource="https://w3id.org/digitalconstruction/0.5/Entities#ContinuantFiatBoundary"/>
            </owl:Restriction>
        </rdfs:subClassOf>
        <rdfs:comment>ContinuantFiatBoundary is equivalent to the BFO class &apos;continuant fiat boundary&apos; (http://purl.obolibrary.org/obo/BFO_0000140)</rdfs:comment>
        <rdfs:label>ContinuantFiatBoundary</rdfs:label>
    </owl:Class>
    


    <!-- https://w3id.org/digitalconstruction/0.5/Entities#Device -->

    <owl:Class rdf:about="https://w3id.org/digitalconstruction/0.5/Entities#Device">
        <rdfs:subClassOf rdf:resource="https://w3id.org/digitalconstruction/0.5/Entities#Object"/>
        <rdfs:comment>An object that performs a function, requiring at most only intermittent control by a user (an agent).

Examples: Sensor, actuator, dishwasher, heater.</rdfs:comment>
        <rdfs:label>Device</rdfs:label>
    </owl:Class>
    


    <!-- https://w3id.org/digitalconstruction/0.5/Entities#Disposition -->

    <owl:Class rdf:about="https://w3id.org/digitalconstruction/0.5/Entities#Disposition">
        <rdfs:subClassOf rdf:resource="https://w3id.org/digitalconstruction/0.5/Entities#RealizableEntity"/>
        <owl:disjointWith rdf:resource="https://w3id.org/digitalconstruction/0.5/Entities#Role"/>
        <rdfs:comment>Disposition is equivalent to the BFO class &apos;disposition&apos; (http://purl.obolibrary.org/obo/BFO_0000016)</rdfs:comment>
        <rdfs:label>Disposition</rdfs:label>
    </owl:Class>
    


    <!-- https://w3id.org/digitalconstruction/0.5/Entities#Entity -->

    <owl:Class rdf:about="https://w3id.org/digitalconstruction/0.5/Entities#Entity">
        <owl:equivalentClass rdf:resource="https://w3id.org/digitalconstruction/0.5/Variables#Subject"/>
        <rdfs:comment>Entity is equivalent to the BFO class &apos;entity&apos; (http://purl.obolibrary.org/obo/BFO_0000001)</rdfs:comment>
        <rdfs:label>Entity</rdfs:label>
    </owl:Class>
    


    <!-- https://w3id.org/digitalconstruction/0.5/Entities#EntityScope -->

    <owl:Class rdf:about="https://w3id.org/digitalconstruction/0.5/Entities#EntityScope">
        <rdfs:subClassOf rdf:resource="https://w3id.org/digitalconstruction/0.5/Entities#Category"/>
        <rdfs:comment>Category that contains all entities in a scope of a given entity. For example, all entities in a system, or within a scope of a plan.</rdfs:comment>
        <rdfs:label>EntityScope</rdfs:label>
    </owl:Class>
    


    <!-- https://w3id.org/digitalconstruction/0.5/Entities#EntityState -->

    <owl:Class rdf:about="https://w3id.org/digitalconstruction/0.5/Entities#EntityState">
        <rdfs:subClassOf rdf:resource="https://w3id.org/digitalconstruction/0.5/Entities#Disposition"/>
        <rdfs:comment>Inherent state of an entity. For instance, possible states for a device are: initial, manufactured, installed, approved, and for a wall: initial, frame constructed, plated, plastered, painted, approved. The move from state to another requires the execution of appropriate activities.</rdfs:comment>
        <rdfs:label>EntityState</rdfs:label>
    </owl:Class>
    


    <!-- https://w3id.org/digitalconstruction/0.5/Entities#Equipment -->

    <owl:Class rdf:about="https://w3id.org/digitalconstruction/0.5/Entities#Equipment">
        <rdfs:subClassOf rdf:resource="https://w3id.org/digitalconstruction/0.5/Entities#Object"/>
        <rdfs:comment>An object needed to perform an activity, and when used is in continuous control of the agent involved in the activity. Equipment cannot execute activities by themselves.

Examples: Vehices, cranes, and tools such as hammers and drills.</rdfs:comment>
        <rdfs:label>Equipment</rdfs:label>
    </owl:Class>
    


    <!-- https://w3id.org/digitalconstruction/0.5/Entities#FiatLine -->

    <owl:Class rdf:about="https://w3id.org/digitalconstruction/0.5/Entities#FiatLine">
        <rdfs:subClassOf rdf:resource="https://w3id.org/digitalconstruction/0.5/Entities#ContinuantFiatBoundary"/>
        <rdfs:subClassOf>
            <owl:Restriction>
                <owl:onProperty rdf:resource="https://w3id.org/digitalconstruction/0.5/Entities#hasContinuantPartAtAllTimes"/>
                <owl:allValuesFrom>
                    <owl:Class>
                        <owl:unionOf rdf:parseType="Collection">
                            <rdf:Description rdf:about="https://w3id.org/digitalconstruction/0.5/Entities#FiatLine"/>
                            <rdf:Description rdf:about="https://w3id.org/digitalconstruction/0.5/Entities#FiatPoint"/>
                        </owl:unionOf>
                    </owl:Class>
                </owl:allValuesFrom>
            </owl:Restriction>
        </rdfs:subClassOf>
        <rdfs:comment>FiatLine is equivalent to the BFO class &apos;fiat line&apos; (http://purl.obolibrary.org/obo/BFO_0000142)</rdfs:comment>
        <rdfs:label>FiatLine</rdfs:label>
    </owl:Class>
    


    <!-- https://w3id.org/digitalconstruction/0.5/Entities#FiatObjectPart -->

    <owl:Class rdf:about="https://w3id.org/digitalconstruction/0.5/Entities#FiatObjectPart">
        <rdfs:subClassOf rdf:resource="https://w3id.org/digitalconstruction/0.5/Entities#MaterialEntity"/>
        <rdfs:comment>FiatObjectPart is equivalent to the BFO class &apos;fiat object part&apos; (http://purl.obolibrary.org/obo/BFO_0000024)</rdfs:comment>
        <rdfs:label>FiatObjectPart</rdfs:label>
    </owl:Class>
    


    <!-- https://w3id.org/digitalconstruction/0.5/Entities#FiatPoint -->

    <owl:Class rdf:about="https://w3id.org/digitalconstruction/0.5/Entities#FiatPoint">
        <rdfs:subClassOf rdf:resource="https://w3id.org/digitalconstruction/0.5/Entities#ContinuantFiatBoundary"/>
        <rdfs:subClassOf>
            <owl:Restriction>
                <owl:onProperty rdf:resource="https://w3id.org/digitalconstruction/0.5/Entities#hasContinuantPartAtAllTimes"/>
                <owl:allValuesFrom rdf:resource="https://w3id.org/digitalconstruction/0.5/Entities#FiatPoint"/>
            </owl:Restriction>
        </rdfs:subClassOf>
        <rdfs:comment>FiatPoint is equivalent to the BFO class &apos;fiat point&apos; (http://purl.obolibrary.org/obo/BFO_0000147)</rdfs:comment>
        <rdfs:label>FiatPoint</rdfs:label>
    </owl:Class>
    


    <!-- https://w3id.org/digitalconstruction/0.5/Entities#FiatSurface -->

    <owl:Class rdf:about="https://w3id.org/digitalconstruction/0.5/Entities#FiatSurface">
        <rdfs:subClassOf rdf:resource="https://w3id.org/digitalconstruction/0.5/Entities#ContinuantFiatBoundary"/>
        <rdfs:subClassOf>
            <owl:Restriction>
                <owl:onProperty rdf:resource="https://w3id.org/digitalconstruction/0.5/Entities#hasContinuantPartAtAllTimes"/>
                <owl:allValuesFrom rdf:resource="https://w3id.org/digitalconstruction/0.5/Entities#ContinuantFiatBoundary"/>
            </owl:Restriction>
        </rdfs:subClassOf>
        <rdfs:comment>FiatSurface is equivalent to the BFO class &apos;fiat surface&apos; (http://purl.obolibrary.org/obo/BFO_0000146)</rdfs:comment>
        <rdfs:label>FiatSurface</rdfs:label>
    </owl:Class>
    


    <!-- https://w3id.org/digitalconstruction/0.5/Entities#Function -->

    <owl:Class rdf:about="https://w3id.org/digitalconstruction/0.5/Entities#Function">
        <rdfs:subClassOf rdf:resource="https://w3id.org/digitalconstruction/0.5/Entities#Disposition"/>
        <rdfs:comment>Function is equivalent to the BFO class &apos;function&apos; (http://purl.obolibrary.org/obo/BFO_0000034)</rdfs:comment>
        <rdfs:label>Function</rdfs:label>
    </owl:Class>
    


    <!-- https://w3id.org/digitalconstruction/0.5/Entities#GenericallyDependentContinuant -->

    <owl:Class rdf:about="https://w3id.org/digitalconstruction/0.5/Entities#GenericallyDependentContinuant">
        <rdfs:subClassOf rdf:resource="https://w3id.org/digitalconstruction/0.5/Entities#Continuant"/>
        <rdfs:comment>GenericallyDependentContinuant is equivalent to the BFO class &apos;generically dependent continuant&apos; (http://purl.obolibrary.org/obo/BFO_0000031)</rdfs:comment>
        <rdfs:label>GenericallyDependentContinuant</rdfs:label>
    </owl:Class>
    


    <!-- https://w3id.org/digitalconstruction/0.5/Entities#GeodeticBoundingBox -->

    <owl:Class rdf:about="https://w3id.org/digitalconstruction/0.5/Entities#GeodeticBoundingBox">
        <rdfs:subClassOf rdf:resource="https://w3id.org/digitalconstruction/0.5/Entities#SpatialExtent"/>
        <rdfs:comment>Minimum bounding box of a geodetic area determined by its minimum geodetic position and maximum geodetic position</rdfs:comment>
        <rdfs:label>GeodeticBoundingBox</rdfs:label>
    </owl:Class>
    


    <!-- https://w3id.org/digitalconstruction/0.5/Entities#GeodeticPosition -->

    <owl:Class rdf:about="https://w3id.org/digitalconstruction/0.5/Entities#GeodeticPosition">
        <rdfs:subClassOf rdf:resource="https://w3id.org/digitalconstruction/0.5/Entities#SpatialPosition"/>
        <rdfs:comment>Geodetic position expressed in longitude, latitude and altitude with respect to a geodetic coordinate system.</rdfs:comment>
        <rdfs:label>GeodeticPosition</rdfs:label>
    </owl:Class>
    


    <!-- https://w3id.org/digitalconstruction/0.5/Entities#Group -->

    <owl:Class rdf:about="https://w3id.org/digitalconstruction/0.5/Entities#Group">
        <rdfs:subClassOf rdf:resource="https://w3id.org/digitalconstruction/0.5/Entities#Entity"/>
        <rdfs:comment>A set of entities. Examples are sets created for management purposes, such as a procurement package, a cost control item, a shipment, a material kit, a workgroup, or the walls of a space. One group may contain entities belonging to otherwise disjoint fundamental categories, such as material batches, equipment, information content entities, and activities.</rdfs:comment>
        <rdfs:label>Group</rdfs:label>
    </owl:Class>
    


    <!-- https://w3id.org/digitalconstruction/0.5/Entities#History -->

    <owl:Class rdf:about="https://w3id.org/digitalconstruction/0.5/Entities#History">
        <rdfs:subClassOf rdf:resource="https://w3id.org/digitalconstruction/0.5/Entities#Process"/>
        <rdfs:comment>History is equivalent to the BFO class &apos;history&apos; (http://purl.obolibrary.org/obo/BFO_0000182)</rdfs:comment>
        <rdfs:label>History</rdfs:label>
    </owl:Class>
    


    <!-- https://w3id.org/digitalconstruction/0.5/Entities#Identifier -->

    <owl:Class rdf:about="https://w3id.org/digitalconstruction/0.5/Entities#Identifier">
        <rdfs:subClassOf rdf:resource="https://w3id.org/digitalconstruction/0.5/Entities#Labeling"/>
        <rdfs:comment>A specifier of a global or local identity of an entity, in a given identification scope. Examples are a GUID, a GTIN, a social security number, a room number within a building, a control point number in a building automatization system.</rdfs:comment>
        <rdfs:label>Identifier</rdfs:label>
    </owl:Class>
    


    <!-- https://w3id.org/digitalconstruction/0.5/Entities#ImmaterialEntity -->

    <owl:Class rdf:about="https://w3id.org/digitalconstruction/0.5/Entities#ImmaterialEntity">
        <rdfs:subClassOf rdf:resource="https://w3id.org/digitalconstruction/0.5/Entities#IndependentContinuant"/>
        <owl:disjointWith rdf:resource="https://w3id.org/digitalconstruction/0.5/Entities#MaterialEntity"/>
        <rdfs:comment>ImmaterialEntity is equivalent to the BFO class &apos;immaterial entity&apos; (http://purl.obolibrary.org/obo/BFO_0000141)</rdfs:comment>
        <rdfs:label>ImmaterialEntity</rdfs:label>
    </owl:Class>
    


    <!-- https://w3id.org/digitalconstruction/0.5/Entities#IndependentContinuant -->

    <owl:Class rdf:about="https://w3id.org/digitalconstruction/0.5/Entities#IndependentContinuant">
        <rdfs:subClassOf rdf:resource="https://w3id.org/digitalconstruction/0.5/Entities#Continuant"/>
        <rdfs:subClassOf>
            <owl:Restriction>
                <owl:onProperty rdf:resource="https://w3id.org/digitalconstruction/0.5/Entities#continuantPartOfAtAllTimes"/>
                <owl:allValuesFrom rdf:resource="https://w3id.org/digitalconstruction/0.5/Entities#IndependentContinuant"/>
            </owl:Restriction>
        </rdfs:subClassOf>
        <rdfs:comment>IndependentContinuant is equivalent to the BFO class &apos;independent continuant&apos; (http://purl.obolibrary.org/obo/BFO_0000004)</rdfs:comment>
        <rdfs:label>IndependentContinuant</rdfs:label>
    </owl:Class>
    


    <!-- https://w3id.org/digitalconstruction/0.5/Entities#Labeling -->

    <owl:Class rdf:about="https://w3id.org/digitalconstruction/0.5/Entities#Labeling">
        <rdfs:subClassOf rdf:resource="https://w3id.org/digitalconstruction/0.5/Entities#Quality"/>
        <rdfs:comment>Labeling is a generic mechanism to associate entities with any number of labels that are unique within a given category. The purpose is to enable the representation of connections to existing systems, databases or classification schemes.</rdfs:comment>
        <rdfs:label>Labeling</rdfs:label>
    </owl:Class>
    


    <!-- https://w3id.org/digitalconstruction/0.5/Entities#Location -->

    <owl:Class rdf:about="https://w3id.org/digitalconstruction/0.5/Entities#Location">
        <rdfs:subClassOf rdf:resource="https://w3id.org/digitalconstruction/0.5/Entities#Site"/>
        <rdfs:comment>A (logical) place where material entities can be located or activities can occur. Locations can form a hierarchy, for example, in a location breakdown structure consisting of a site, buildings, floors, zones, spaces, and workspaces</rdfs:comment>
        <rdfs:label>Location</rdfs:label>
    </owl:Class>
    


    <!-- https://w3id.org/digitalconstruction/0.5/Entities#MaterialEntity -->

    <owl:Class rdf:about="https://w3id.org/digitalconstruction/0.5/Entities#MaterialEntity">
        <rdfs:subClassOf rdf:resource="https://w3id.org/digitalconstruction/0.5/Entities#IndependentContinuant"/>
        <rdfs:subClassOf>
            <owl:Restriction>
                <owl:onProperty rdf:resource="https://w3id.org/digitalconstruction/0.5/Entities#continuantPartOfAtAllTimes"/>
                <owl:allValuesFrom rdf:resource="https://w3id.org/digitalconstruction/0.5/Entities#MaterialEntity"/>
            </owl:Restriction>
        </rdfs:subClassOf>
        <rdfs:subClassOf>
            <owl:Restriction>
                <owl:onProperty rdf:resource="https://w3id.org/digitalconstruction/0.5/Entities#hasContinuantPartAtAllTimes"/>
                <owl:allValuesFrom>
                    <owl:Class>
                        <owl:unionOf rdf:parseType="Collection">
                            <rdf:Description rdf:about="https://w3id.org/digitalconstruction/0.5/Entities#ContinuantFiatBoundary"/>
                            <rdf:Description rdf:about="https://w3id.org/digitalconstruction/0.5/Entities#MaterialEntity"/>
                            <rdf:Description rdf:about="https://w3id.org/digitalconstruction/0.5/Entities#Site"/>
                        </owl:unionOf>
                    </owl:Class>
                </owl:allValuesFrom>
            </owl:Restriction>
        </rdfs:subClassOf>
        <rdfs:comment>MaterialEntity is equivalent to the BFO class &apos;material entity&apos; (http://purl.obolibrary.org/obo/BFO_0000040)</rdfs:comment>
        <rdfs:label>MaterialEntity</rdfs:label>
    </owl:Class>
    


    <!-- https://w3id.org/digitalconstruction/0.5/Entities#NonResidentialUnit -->

    <owl:Class rdf:about="https://w3id.org/digitalconstruction/0.5/Entities#NonResidentialUnit">
        <rdfs:subClassOf rdf:resource="https://w3id.org/digitalconstruction/0.5/Entities#BuildingUnit"/>
        <rdfs:comment>A building unit used for purposes other than living, such as commercial,  service or storage functions.</rdfs:comment>
        <rdfs:label>NonResidentialUnit</rdfs:label>
    </owl:Class>
    


    <!-- https://w3id.org/digitalconstruction/0.5/Entities#Object -->

    <owl:Class rdf:about="https://w3id.org/digitalconstruction/0.5/Entities#Object">
        <rdfs:subClassOf rdf:resource="https://w3id.org/digitalconstruction/0.5/Entities#MaterialEntity"/>
        <rdfs:comment>Object is equivalent to the BFO class &apos;object&apos; (http://purl.obolibrary.org/obo/BFO_0000030)</rdfs:comment>
        <rdfs:label>Object</rdfs:label>
    </owl:Class>
    


    <!-- https://w3id.org/digitalconstruction/0.5/Entities#ObjectAggregate -->

    <owl:Class rdf:about="https://w3id.org/digitalconstruction/0.5/Entities#ObjectAggregate">
        <rdfs:subClassOf rdf:resource="https://w3id.org/digitalconstruction/0.5/Entities#MaterialEntity"/>
        <rdfs:comment>ObjectAggregate is equivalent to the BFO class &apos;object aggregate&apos; (http://purl.obolibrary.org/obo/BFO_0000027)</rdfs:comment>
        <rdfs:label>ObjectAggregate</rdfs:label>
    </owl:Class>
    


    <!-- https://w3id.org/digitalconstruction/0.5/Entities#Occurrent -->

    <owl:Class rdf:about="https://w3id.org/digitalconstruction/0.5/Entities#Occurrent">
        <rdfs:subClassOf rdf:resource="https://w3id.org/digitalconstruction/0.5/Entities#Entity"/>
        <rdfs:comment>Occurrent is equivalent to the BFO class &apos;occurrent&apos; (http://purl.obolibrary.org/obo/BFO_0000003)</rdfs:comment>
        <rdfs:label>Occurrent</rdfs:label>
    </owl:Class>
    


    <!-- https://w3id.org/digitalconstruction/0.5/Entities#OneAngleOrientation -->

    <owl:Class rdf:about="https://w3id.org/digitalconstruction/0.5/Entities#OneAngleOrientation">
        <rdfs:subClassOf rdf:resource="https://w3id.org/digitalconstruction/0.5/Entities#SpatialOrientation"/>
        <rdfs:comment>Orientation in two dimensions given by the orientation angle from true north</rdfs:comment>
        <rdfs:label>OneAngleOrientation</rdfs:label>
    </owl:Class>
    


    <!-- https://w3id.org/digitalconstruction/0.5/Entities#OneDimensionalSpatialRegion -->

    <owl:Class rdf:about="https://w3id.org/digitalconstruction/0.5/Entities#OneDimensionalSpatialRegion">
        <rdfs:subClassOf rdf:resource="https://w3id.org/digitalconstruction/0.5/Entities#SpatialRegion"/>
        <rdfs:subClassOf>
            <owl:Restriction>
                <owl:onProperty rdf:resource="https://w3id.org/digitalconstruction/0.5/Entities#hasContinuantPartAtAllTimes"/>
                <owl:allValuesFrom>
                    <owl:Class>
                        <owl:unionOf rdf:parseType="Collection">
                            <rdf:Description rdf:about="https://w3id.org/digitalconstruction/0.5/Entities#OneDimensionalSpatialRegion"/>
                            <rdf:Description rdf:about="https://w3id.org/digitalconstruction/0.5/Entities#ZeroDimensionalSpatialRegion"/>
                        </owl:unionOf>
                    </owl:Class>
                </owl:allValuesFrom>
            </owl:Restriction>
        </rdfs:subClassOf>
        <rdfs:comment>OneDimensionalSpatialRegion is equivalent to the BFO class &apos;one-dimensional spatial region&apos; (http://purl.obolibrary.org/obo/BFO_0000026)</rdfs:comment>
        <rdfs:label>OneDimensionalSpatialRegion</rdfs:label>
    </owl:Class>
    


    <!-- https://w3id.org/digitalconstruction/0.5/Entities#OneDimensionalTemporalRegion -->

    <owl:Class rdf:about="https://w3id.org/digitalconstruction/0.5/Entities#OneDimensionalTemporalRegion">
        <rdfs:subClassOf rdf:resource="https://w3id.org/digitalconstruction/0.5/Entities#TemporalRegion"/>
        <rdfs:subClassOf>
            <owl:Restriction>
                <owl:onProperty rdf:resource="https://w3id.org/digitalconstruction/0.5/Entities#hasTemporalPart"/>
                <owl:allValuesFrom>
                    <owl:Class>
                        <owl:unionOf rdf:parseType="Collection">
                            <rdf:Description rdf:about="https://w3id.org/digitalconstruction/0.5/Entities#OneDimensionalTemporalRegion"/>
                            <rdf:Description rdf:about="https://w3id.org/digitalconstruction/0.5/Entities#ZeroDimensionalTemporalRegion"/>
                        </owl:unionOf>
                    </owl:Class>
                </owl:allValuesFrom>
            </owl:Restriction>
        </rdfs:subClassOf>
        <rdfs:subClassOf>
            <owl:Restriction>
                <owl:onProperty rdf:resource="https://w3id.org/digitalconstruction/0.5/Entities#temporalPartOf"/>
                <owl:allValuesFrom rdf:resource="https://w3id.org/digitalconstruction/0.5/Entities#OneDimensionalTemporalRegion"/>
            </owl:Restriction>
        </rdfs:subClassOf>
        <owl:disjointWith rdf:resource="https://w3id.org/digitalconstruction/0.5/Entities#ZeroDimensionalTemporalRegion"/>
        <rdfs:comment>OneDimensionalTemporalRegion is equivalent to the BFO class &apos;one-dimensional temporal region&apos; (http://purl.obolibrary.org/obo/BFO_0000038)</rdfs:comment>
        <rdfs:label>OneDimensionalTemporalRegion</rdfs:label>
    </owl:Class>
    


    <!-- https://w3id.org/digitalconstruction/0.5/Entities#Process -->

    <owl:Class rdf:about="https://w3id.org/digitalconstruction/0.5/Entities#Process">
        <rdfs:subClassOf rdf:resource="https://w3id.org/digitalconstruction/0.5/Entities#Occurrent"/>
        <rdfs:subClassOf>
            <owl:Restriction>
                <owl:onProperty rdf:resource="https://w3id.org/digitalconstruction/0.5/Entities#hasOccurrentPart"/>
                <owl:allValuesFrom>
                    <owl:Class>
                        <owl:unionOf rdf:parseType="Collection">
                            <rdf:Description rdf:about="https://w3id.org/digitalconstruction/0.5/Entities#Process"/>
                            <rdf:Description rdf:about="https://w3id.org/digitalconstruction/0.5/Entities#ProcessBoundary"/>
                        </owl:unionOf>
                    </owl:Class>
                </owl:allValuesFrom>
            </owl:Restriction>
        </rdfs:subClassOf>
        <rdfs:subClassOf>
            <owl:Restriction>
                <owl:onProperty rdf:resource="https://w3id.org/digitalconstruction/0.5/Entities#occurrentPartOf"/>
                <owl:allValuesFrom rdf:resource="https://w3id.org/digitalconstruction/0.5/Entities#Process"/>
            </owl:Restriction>
        </rdfs:subClassOf>
        <rdfs:comment>Process is equivalent to the BFO class &apos;process&apos; (http://purl.obolibrary.org/obo/BFO_0000015)</rdfs:comment>
        <rdfs:label>Process</rdfs:label>
    </owl:Class>
    


    <!-- https://w3id.org/digitalconstruction/0.5/Entities#ProcessBoundary -->

    <owl:Class rdf:about="https://w3id.org/digitalconstruction/0.5/Entities#ProcessBoundary">
        <rdfs:subClassOf rdf:resource="https://w3id.org/digitalconstruction/0.5/Entities#Occurrent"/>
        <rdfs:subClassOf>
            <owl:Restriction>
                <owl:onProperty rdf:resource="https://w3id.org/digitalconstruction/0.5/Entities#hasOccurrentPart"/>
                <owl:allValuesFrom rdf:resource="https://w3id.org/digitalconstruction/0.5/Entities#ProcessBoundary"/>
            </owl:Restriction>
        </rdfs:subClassOf>
        <rdfs:subClassOf>
            <owl:Restriction>
                <owl:onProperty rdf:resource="https://w3id.org/digitalconstruction/0.5/Entities#hasTemporalPart"/>
                <owl:allValuesFrom rdf:resource="https://w3id.org/digitalconstruction/0.5/Entities#ProcessBoundary"/>
            </owl:Restriction>
        </rdfs:subClassOf>
        <rdfs:subClassOf>
            <owl:Restriction>
                <owl:onProperty rdf:resource="https://w3id.org/digitalconstruction/0.5/Entities#occurrentPartOf"/>
                <owl:allValuesFrom>
                    <owl:Class>
                        <owl:unionOf rdf:parseType="Collection">
                            <rdf:Description rdf:about="https://w3id.org/digitalconstruction/0.5/Entities#Process"/>
                            <rdf:Description rdf:about="https://w3id.org/digitalconstruction/0.5/Entities#ProcessBoundary"/>
                        </owl:unionOf>
                    </owl:Class>
                </owl:allValuesFrom>
            </owl:Restriction>
        </rdfs:subClassOf>
        <rdfs:comment>ProcessBoundary is equivalent to the BFO class &apos;process boundary&apos; (http://purl.obolibrary.org/obo/BFO_0000035)</rdfs:comment>
        <rdfs:label>ProcessBoundary</rdfs:label>
    </owl:Class>
    


    <!-- https://w3id.org/digitalconstruction/0.5/Entities#Quality -->

    <owl:Class rdf:about="https://w3id.org/digitalconstruction/0.5/Entities#Quality">
        <rdfs:subClassOf rdf:resource="https://w3id.org/digitalconstruction/0.5/Entities#SpecificallyDependentContinuant"/>
        <rdfs:subClassOf rdf:resource="https://w3id.org/digitalconstruction/0.5/Variables#Property"/>
        <owl:disjointWith rdf:resource="https://w3id.org/digitalconstruction/0.5/Entities#RealizableEntity"/>
        <rdfs:comment>Quality is equivalent to the BFO class &apos;quality&apos; (http://purl.obolibrary.org/obo/BFO_0000019)</rdfs:comment>
        <rdfs:label>Quality</rdfs:label>
    </owl:Class>
    


    <!-- https://w3id.org/digitalconstruction/0.5/Entities#RealEstate -->

    <owl:Class rdf:about="https://w3id.org/digitalconstruction/0.5/Entities#RealEstate">
        <rdfs:subClassOf rdf:resource="https://w3id.org/digitalconstruction/0.5/Entities#BuiltAsset"/>
        <rdfs:comment>A property consisting of land or buildings.</rdfs:comment>
        <rdfs:label>RealEstate</rdfs:label>
    </owl:Class>
    


    <!-- https://w3id.org/digitalconstruction/0.5/Entities#RealizableEntity -->

    <owl:Class rdf:about="https://w3id.org/digitalconstruction/0.5/Entities#RealizableEntity">
        <rdfs:subClassOf rdf:resource="https://w3id.org/digitalconstruction/0.5/Entities#SpecificallyDependentContinuant"/>
        <rdfs:comment>RealizableEntity is equivalent to the BFO class &apos;realizable entity&apos; (http://purl.obolibrary.org/obo/BFO_0000017)</rdfs:comment>
        <rdfs:label>RealizableEntity</rdfs:label>
    </owl:Class>
    


    <!-- https://w3id.org/digitalconstruction/0.5/Entities#RelationalQuality -->

    <owl:Class rdf:about="https://w3id.org/digitalconstruction/0.5/Entities#RelationalQuality">
        <rdfs:subClassOf rdf:resource="https://w3id.org/digitalconstruction/0.5/Entities#Quality"/>
        <rdfs:comment>RelationalQuality is equivalent to the BFO class &apos;relational quality&apos; (http://purl.obolibrary.org/obo/BFO_0000145)</rdfs:comment>
        <rdfs:label>RelationalQuality</rdfs:label>
    </owl:Class>
    


    <!-- https://w3id.org/digitalconstruction/0.5/Entities#ResidentialUnit -->

    <owl:Class rdf:about="https://w3id.org/digitalconstruction/0.5/Entities#ResidentialUnit">
        <rdfs:subClassOf rdf:resource="https://w3id.org/digitalconstruction/0.5/Entities#BuildingUnit"/>
        <rdfs:comment>A building unit that is used as a residence.

Examples: apartment, condomium, studio.</rdfs:comment>
        <rdfs:label>ResidentialUnit</rdfs:label>
    </owl:Class>
    


    <!-- https://w3id.org/digitalconstruction/0.5/Entities#Role -->

    <owl:Class rdf:about="https://w3id.org/digitalconstruction/0.5/Entities#Role">
        <rdfs:subClassOf rdf:resource="https://w3id.org/digitalconstruction/0.5/Entities#RealizableEntity"/>
        <rdfs:comment>Role is equivalent to the BFO class &apos;role&apos; (http://purl.obolibrary.org/obo/BFO_0000023)</rdfs:comment>
        <rdfs:label>Role</rdfs:label>
    </owl:Class>
    


    <!-- https://w3id.org/digitalconstruction/0.5/Entities#Sensor -->

    <owl:Class rdf:about="https://w3id.org/digitalconstruction/0.5/Entities#Sensor">
        <rdfs:subClassOf rdf:resource="https://w3id.org/digitalconstruction/0.5/Entities#Device"/>
        <rdfs:comment>A device that is capable of producing information about its environment.</rdfs:comment>
        <rdfs:label>Sensor</rdfs:label>
    </owl:Class>
    


    <!-- https://w3id.org/digitalconstruction/0.5/Entities#Site -->

    <owl:Class rdf:about="https://w3id.org/digitalconstruction/0.5/Entities#Site">
        <rdfs:subClassOf rdf:resource="https://w3id.org/digitalconstruction/0.5/Entities#ImmaterialEntity"/>
        <rdfs:subClassOf>
            <owl:Restriction>
                <owl:onProperty rdf:resource="https://w3id.org/digitalconstruction/0.5/Entities#continuantPartOfAtAllTimes"/>
                <owl:allValuesFrom>
                    <owl:Class>
                        <owl:unionOf rdf:parseType="Collection">
                            <rdf:Description rdf:about="https://w3id.org/digitalconstruction/0.5/Entities#MaterialEntity"/>
                            <rdf:Description rdf:about="https://w3id.org/digitalconstruction/0.5/Entities#Site"/>
                        </owl:unionOf>
                    </owl:Class>
                </owl:allValuesFrom>
            </owl:Restriction>
        </rdfs:subClassOf>
        <rdfs:subClassOf>
            <owl:Restriction>
                <owl:onProperty rdf:resource="https://w3id.org/digitalconstruction/0.5/Entities#hasContinuantPartAtAllTimes"/>
                <owl:allValuesFrom>
                    <owl:Class>
                        <owl:unionOf rdf:parseType="Collection">
                            <rdf:Description rdf:about="https://w3id.org/digitalconstruction/0.5/Entities#ContinuantFiatBoundary"/>
                            <rdf:Description rdf:about="https://w3id.org/digitalconstruction/0.5/Entities#Site"/>
                        </owl:unionOf>
                    </owl:Class>
                </owl:allValuesFrom>
            </owl:Restriction>
        </rdfs:subClassOf>
        <rdfs:subClassOf>
            <owl:Restriction>
                <owl:onProperty rdf:resource="https://w3id.org/digitalconstruction/0.5/Entities#occupiesSpatialRegionAtAllTimes"/>
                <owl:allValuesFrom rdf:resource="https://w3id.org/digitalconstruction/0.5/Entities#ThreeDimensionalSpatialRegion"/>
            </owl:Restriction>
        </rdfs:subClassOf>
        <rdfs:comment>Site is equivalent to the BFO class &apos;site&apos; (http://purl.obolibrary.org/obo/BFO_0000029)</rdfs:comment>
        <rdfs:label>Site</rdfs:label>
    </owl:Class>
    


    <!-- https://w3id.org/digitalconstruction/0.5/Entities#SpatialExtent -->

    <owl:Class rdf:about="https://w3id.org/digitalconstruction/0.5/Entities#SpatialExtent">
        <rdfs:subClassOf rdf:resource="https://w3id.org/digitalconstruction/0.5/Entities#SpatialQuality"/>
        <rdfs:comment>The dimensions of a spatial region</rdfs:comment>
        <rdfs:label>SpatialExtent</rdfs:label>
    </owl:Class>
    


    <!-- https://w3id.org/digitalconstruction/0.5/Entities#SpatialOrientation -->

    <owl:Class rdf:about="https://w3id.org/digitalconstruction/0.5/Entities#SpatialOrientation">
        <rdfs:subClassOf rdf:resource="https://w3id.org/digitalconstruction/0.5/Entities#SpatialQuality"/>
        <rdfs:label>SpatialOrientation</rdfs:label>
    </owl:Class>
    


    <!-- https://w3id.org/digitalconstruction/0.5/Entities#SpatialPosition -->

    <owl:Class rdf:about="https://w3id.org/digitalconstruction/0.5/Entities#SpatialPosition">
        <rdfs:subClassOf rdf:resource="https://w3id.org/digitalconstruction/0.5/Entities#SpatialQuality"/>
        <rdfs:comment>A position in a space</rdfs:comment>
        <rdfs:label>SpatialPosition</rdfs:label>
    </owl:Class>
    


    <!-- https://w3id.org/digitalconstruction/0.5/Entities#SpatialQuality -->

    <owl:Class rdf:about="https://w3id.org/digitalconstruction/0.5/Entities#SpatialQuality">
        <rdfs:subClassOf rdf:resource="https://w3id.org/digitalconstruction/0.5/Entities#Quality"/>
        <rdfs:comment>A quality that concerns the spatial aspects of an entity</rdfs:comment>
        <rdfs:label>SpatialQuality</rdfs:label>
    </owl:Class>
    


    <!-- https://w3id.org/digitalconstruction/0.5/Entities#SpatialRegion -->

    <owl:Class rdf:about="https://w3id.org/digitalconstruction/0.5/Entities#SpatialRegion">
        <rdfs:subClassOf rdf:resource="https://w3id.org/digitalconstruction/0.5/Entities#ImmaterialEntity"/>
        <rdfs:subClassOf>
            <owl:Restriction>
                <owl:onProperty rdf:resource="https://w3id.org/digitalconstruction/0.5/Entities#continuantPartOfAtAllTimes"/>
                <owl:allValuesFrom rdf:resource="https://w3id.org/digitalconstruction/0.5/Entities#SpatialRegion"/>
            </owl:Restriction>
        </rdfs:subClassOf>
        <rdfs:comment>SpatialRegion is equivalent to the BFO class &apos;spatial region&apos; (http://purl.obolibrary.org/obo/BFO_0000006)</rdfs:comment>
        <rdfs:label>SpatialRegion</rdfs:label>
    </owl:Class>
    


    <!-- https://w3id.org/digitalconstruction/0.5/Entities#SpatiotemporalRegion -->

    <owl:Class rdf:about="https://w3id.org/digitalconstruction/0.5/Entities#SpatiotemporalRegion">
        <rdfs:subClassOf rdf:resource="https://w3id.org/digitalconstruction/0.5/Entities#Occurrent"/>
        <rdfs:subClassOf>
            <owl:Restriction>
                <owl:onProperty rdf:resource="https://w3id.org/digitalconstruction/0.5/Entities#occurrentPartOf"/>
                <owl:allValuesFrom rdf:resource="https://w3id.org/digitalconstruction/0.5/Entities#SpatiotemporalRegion"/>
            </owl:Restriction>
        </rdfs:subClassOf>
        <rdfs:subClassOf>
            <owl:Restriction>
                <owl:onProperty rdf:resource="https://w3id.org/digitalconstruction/0.5/Entities#temporalPartOf"/>
                <owl:allValuesFrom rdf:resource="https://w3id.org/digitalconstruction/0.5/Entities#SpatiotemporalRegion"/>
            </owl:Restriction>
        </rdfs:subClassOf>
        <rdfs:comment>SpatiotemporalRegion is equivalent to the BFO class &apos;spatiotemporal region&apos; (http://purl.obolibrary.org/obo/BFO_0000011)</rdfs:comment>
        <rdfs:label>SpatiotemporalRegion</rdfs:label>
    </owl:Class>
    


    <!-- https://w3id.org/digitalconstruction/0.5/Entities#SpecificallyDependentContinuant -->

    <owl:Class rdf:about="https://w3id.org/digitalconstruction/0.5/Entities#SpecificallyDependentContinuant">
        <rdfs:subClassOf rdf:resource="https://w3id.org/digitalconstruction/0.5/Entities#Continuant"/>
        <rdfs:comment>SpecificallyDependentContinuant is equivalent to the BFO class &apos;specifically dependent continuant&apos; (http://purl.obolibrary.org/obo/BFO_0000020)</rdfs:comment>
        <rdfs:label>SpecificallyDependentContinuant</rdfs:label>
    </owl:Class>
    


    <!-- https://w3id.org/digitalconstruction/0.5/Entities#TemporalQuality -->

    <owl:Class rdf:about="https://w3id.org/digitalconstruction/0.5/Entities#TemporalQuality">
        <rdfs:subClassOf rdf:resource="https://w3id.org/digitalconstruction/0.5/Entities#Quality"/>
        <rdfs:label>TemporalQuality</rdfs:label>
    </owl:Class>
    


    <!-- https://w3id.org/digitalconstruction/0.5/Entities#TemporalRegion -->

    <owl:Class rdf:about="https://w3id.org/digitalconstruction/0.5/Entities#TemporalRegion">
        <rdfs:subClassOf rdf:resource="https://w3id.org/digitalconstruction/0.5/Entities#Occurrent"/>
        <rdfs:subClassOf>
            <owl:Restriction>
                <owl:onProperty rdf:resource="https://w3id.org/digitalconstruction/0.5/Entities#occurrentPartOf"/>
                <owl:allValuesFrom rdf:resource="https://w3id.org/digitalconstruction/0.5/Entities#TemporalRegion"/>
            </owl:Restriction>
        </rdfs:subClassOf>
        <rdfs:subClassOf>
            <owl:Restriction>
                <owl:onProperty rdf:resource="https://w3id.org/digitalconstruction/0.5/Entities#temporalPartOf"/>
                <owl:allValuesFrom rdf:resource="https://w3id.org/digitalconstruction/0.5/Entities#TemporalRegion"/>
            </owl:Restriction>
        </rdfs:subClassOf>
        <rdfs:comment>TemporalRegion is equivalent to the BFO class &apos;temporal region&apos; (http://purl.obolibrary.org/obo/BFO_0000008)</rdfs:comment>
        <rdfs:label>TemporalRegion</rdfs:label>
    </owl:Class>
    


    <!-- https://w3id.org/digitalconstruction/0.5/Entities#ThreeAngleOrientation -->

    <owl:Class rdf:about="https://w3id.org/digitalconstruction/0.5/Entities#ThreeAngleOrientation">
        <rdfs:subClassOf rdf:resource="https://w3id.org/digitalconstruction/0.5/Entities#SpatialOrientation"/>
        <rdfs:comment>Orientation given by three angles: angle about x-axis (alpha), angle about y-axis(beta) and angle about z-axis (gamma)</rdfs:comment>
        <rdfs:label>ThreeAngleOrientation</rdfs:label>
    </owl:Class>
    


    <!-- https://w3id.org/digitalconstruction/0.5/Entities#ThreeDimensionalSpatialRegion -->

    <owl:Class rdf:about="https://w3id.org/digitalconstruction/0.5/Entities#ThreeDimensionalSpatialRegion">
        <rdfs:subClassOf rdf:resource="https://w3id.org/digitalconstruction/0.5/Entities#SpatialRegion"/>
        <rdfs:subClassOf>
            <owl:Restriction>
                <owl:onProperty rdf:resource="https://w3id.org/digitalconstruction/0.5/Entities#hasContinuantPartAtAllTimes"/>
                <owl:allValuesFrom rdf:resource="https://w3id.org/digitalconstruction/0.5/Entities#SpatialRegion"/>
            </owl:Restriction>
        </rdfs:subClassOf>
        <rdfs:comment>ThreeDimensionalSpatialRegion is equivalent to the BFO class &apos;three-dimensional spatial region&apos; (http://purl.obolibrary.org/obo/BFO_0000028)</rdfs:comment>
        <rdfs:label>ThreeDimensionalSpatialRegion</rdfs:label>
    </owl:Class>
    


    <!-- https://w3id.org/digitalconstruction/0.5/Entities#TimeDuration -->

    <owl:Class rdf:about="https://w3id.org/digitalconstruction/0.5/Entities#TimeDuration">
        <rdfs:subClassOf rdf:resource="https://w3id.org/digitalconstruction/0.5/Entities#TemporalQuality"/>
        <rdfs:label>TimeDuration</rdfs:label>
    </owl:Class>
    


    <!-- https://w3id.org/digitalconstruction/0.5/Entities#TimeInstant -->

    <owl:Class rdf:about="https://w3id.org/digitalconstruction/0.5/Entities#TimeInstant">
        <rdfs:subClassOf rdf:resource="https://w3id.org/digitalconstruction/0.5/Entities#ZeroDimensionalTemporalRegion"/>
        <rdfs:comment>TimeInstant is equivalent to the BFO class &apos;temporal instant&apos; (http://purl.obolibrary.org/obo/BFO_0000203)</rdfs:comment>
        <rdfs:label>TimeInstant</rdfs:label>
    </owl:Class>
    


    <!-- https://w3id.org/digitalconstruction/0.5/Entities#TimeInterval -->

    <owl:Class rdf:about="https://w3id.org/digitalconstruction/0.5/Entities#TimeInterval">
        <rdfs:subClassOf rdf:resource="https://w3id.org/digitalconstruction/0.5/Entities#OneDimensionalTemporalRegion"/>
        <rdfs:comment>TimeInterval is equivalent to the BFO class &apos;temporal interval&apos; (http://purl.obolibrary.org/obo/BFO_0000202)</rdfs:comment>
        <rdfs:label>TimeInterval</rdfs:label>
    </owl:Class>
    


    <!-- https://w3id.org/digitalconstruction/0.5/Entities#TwoAngleOrientation -->

    <owl:Class rdf:about="https://w3id.org/digitalconstruction/0.5/Entities#TwoAngleOrientation">
        <rdfs:subClassOf rdf:resource="https://w3id.org/digitalconstruction/0.5/Entities#SpatialOrientation"/>
        <rdfs:comment>Orientation of a plane in two dimensions given by its angle about true north (the strike) and the angle of its slope (the dip)</rdfs:comment>
        <rdfs:label>TwoAngleOrientation</rdfs:label>
    </owl:Class>
    


    <!-- https://w3id.org/digitalconstruction/0.5/Entities#TwoDimensionalSpatialRegion -->

    <owl:Class rdf:about="https://w3id.org/digitalconstruction/0.5/Entities#TwoDimensionalSpatialRegion">
        <rdfs:subClassOf rdf:resource="https://w3id.org/digitalconstruction/0.5/Entities#SpatialRegion"/>
        <rdfs:subClassOf>
            <owl:Restriction>
                <owl:onProperty rdf:resource="https://w3id.org/digitalconstruction/0.5/Entities#hasContinuantPartAtAllTimes"/>
                <owl:allValuesFrom>
                    <owl:Class>
                        <owl:unionOf rdf:parseType="Collection">
                            <rdf:Description rdf:about="https://w3id.org/digitalconstruction/0.5/Entities#OneDimensionalSpatialRegion"/>
                            <rdf:Description rdf:about="https://w3id.org/digitalconstruction/0.5/Entities#TwoDimensionalSpatialRegion"/>
                            <rdf:Description rdf:about="https://w3id.org/digitalconstruction/0.5/Entities#ZeroDimensionalSpatialRegion"/>
                        </owl:unionOf>
                    </owl:Class>
                </owl:allValuesFrom>
            </owl:Restriction>
        </rdfs:subClassOf>
        <rdfs:comment>TwoDimensionalSpatialRegion is equivalent to the BFO class &apos;two-dimensional spatial region&apos; (http://purl.obolibrary.org/obo/BFO_0000009)</rdfs:comment>
        <rdfs:label>TwoDimensionalSpatialRegion</rdfs:label>
    </owl:Class>
    


    <!-- https://w3id.org/digitalconstruction/0.5/Entities#Vehicle -->

    <owl:Class rdf:about="https://w3id.org/digitalconstruction/0.5/Entities#Vehicle">
        <rdfs:subClassOf rdf:resource="https://w3id.org/digitalconstruction/0.5/Entities#Equipment"/>
        <rdfs:comment>An equipment for transporting shipments. The vehice also moves from origin to the target of the transportation activity. Examples are trucks or forklifts.</rdfs:comment>
        <rdfs:label>Vehicle</rdfs:label>
    </owl:Class>
    


    <!-- https://w3id.org/digitalconstruction/0.5/Entities#Workspace -->

    <owl:Class rdf:about="https://w3id.org/digitalconstruction/0.5/Entities#Workspace">
        <rdfs:subClassOf rdf:resource="https://w3id.org/digitalconstruction/0.5/Entities#Location"/>
        <rdfs:comment>A site of work. There can be multiple different kinds of workspaces needed by an activity: labor crew space, equipment space, hazard space, and so on.</rdfs:comment>
        <rdfs:label>Workspace</rdfs:label>
    </owl:Class>
    


    <!-- https://w3id.org/digitalconstruction/0.5/Entities#ZeroDimensionalSpatialRegion -->

    <owl:Class rdf:about="https://w3id.org/digitalconstruction/0.5/Entities#ZeroDimensionalSpatialRegion">
        <rdfs:subClassOf rdf:resource="https://w3id.org/digitalconstruction/0.5/Entities#SpatialRegion"/>
        <rdfs:subClassOf>
            <owl:Restriction>
                <owl:onProperty rdf:resource="https://w3id.org/digitalconstruction/0.5/Entities#hasContinuantPartAtAllTimes"/>
                <owl:allValuesFrom rdf:resource="https://w3id.org/digitalconstruction/0.5/Entities#ZeroDimensionalSpatialRegion"/>
            </owl:Restriction>
        </rdfs:subClassOf>
        <rdfs:comment>ZeroDimensionalSpatialRegion is equivalent to the BFO class &apos;zero-dimensional spatial region&apos; (http://purl.obolibrary.org/obo/BFO_0000018)</rdfs:comment>
        <rdfs:label>ZeroDimensionalSpatialRegion</rdfs:label>
    </owl:Class>
    


    <!-- https://w3id.org/digitalconstruction/0.5/Entities#ZeroDimensionalTemporalRegion -->

    <owl:Class rdf:about="https://w3id.org/digitalconstruction/0.5/Entities#ZeroDimensionalTemporalRegion">
        <rdfs:subClassOf rdf:resource="https://w3id.org/digitalconstruction/0.5/Entities#TemporalRegion"/>
        <rdfs:subClassOf>
            <owl:Restriction>
                <owl:onProperty rdf:resource="https://w3id.org/digitalconstruction/0.5/Entities#hasTemporalPart"/>
                <owl:allValuesFrom rdf:resource="https://w3id.org/digitalconstruction/0.5/Entities#ZeroDimensionalTemporalRegion"/>
            </owl:Restriction>
        </rdfs:subClassOf>
        <rdfs:comment>ZeroDimensionalTemporalRegion is equivalent to the BFO class &apos;zero-dimensional temporal region&apos; (http://purl.obolibrary.org/obo/BFO_0000148)</rdfs:comment>
        <rdfs:label>ZeroDimensionalTemporalRegion</rdfs:label>
    </owl:Class>
    


    <!-- https://w3id.org/digitalconstruction/0.5/Variables#Comparison -->

    <owl:Class rdf:about="https://w3id.org/digitalconstruction/0.5/Variables#Comparison">
        <rdfs:subClassOf rdf:resource="https://w3id.org/digitalconstruction/0.5/Entities#RelationalQuality"/>
    </owl:Class>
    


    <!-- https://w3id.org/digitalconstruction/0.5/Variables#Constraint -->

    <owl:Class rdf:about="https://w3id.org/digitalconstruction/0.5/Variables#Constraint">
        <rdfs:subClassOf rdf:resource="https://w3id.org/digitalconstruction/0.5/Entities#RelationalQuality"/>
    </owl:Class>
    


    <!-- https://w3id.org/digitalconstruction/0.5/Variables#Operator -->

    <owl:Class rdf:about="https://w3id.org/digitalconstruction/0.5/Variables#Operator">
        <rdfs:subClassOf rdf:resource="https://w3id.org/digitalconstruction/0.5/Entities#RelationalQuality"/>
    </owl:Class>
    


    <!-- https://w3id.org/digitalconstruction/0.5/Variables#Property -->

    <owl:Class rdf:about="https://w3id.org/digitalconstruction/0.5/Variables#Property"/>
    


    <!-- https://w3id.org/digitalconstruction/0.5/Variables#PropertyState -->

    <owl:Class rdf:about="https://w3id.org/digitalconstruction/0.5/Variables#PropertyState">
        <rdfs:subClassOf rdf:resource="https://w3id.org/digitalconstruction/0.5/Entities#SpecificallyDependentContinuant"/>
    </owl:Class>
    


    <!-- https://w3id.org/digitalconstruction/0.5/Variables#QuantityKind -->

    <owl:Class rdf:about="https://w3id.org/digitalconstruction/0.5/Variables#QuantityKind">
        <rdfs:subClassOf rdf:resource="https://w3id.org/digitalconstruction/0.5/Entities#GenericallyDependentContinuant"/>
    </owl:Class>
    


    <!-- https://w3id.org/digitalconstruction/0.5/Variables#Subject -->

    <owl:Class rdf:about="https://w3id.org/digitalconstruction/0.5/Variables#Subject"/>
    


    <!-- 
    ///////////////////////////////////////////////////////////////////////////////////////
    //
    // General axioms
    //
    ///////////////////////////////////////////////////////////////////////////////////////
     -->

    <rdf:Description>
        <rdf:type rdf:resource="http://www.w3.org/2002/07/owl#AllDisjointClasses"/>
        <owl:members rdf:parseType="Collection">
            <rdf:Description rdf:about="https://w3id.org/digitalconstruction/0.5/Entities#BuildingObject"/>
            <rdf:Description rdf:about="https://w3id.org/digitalconstruction/0.5/Entities#Equipment"/>
            <rdf:Description rdf:about="https://w3id.org/digitalconstruction/0.5/Entities#Location"/>
        </owl:members>
    </rdf:Description>
</rdf:RDF>



<!-- Generated by the OWL API (version 4.5.25.2023-02-15T19:15:49Z) https://github.com/owlcs/owlapi -->

